\subsection{Solutions}
\begin{multicols}{2}
\begin{enumerate}[label={\textbf{\arabic*.}}]
\item \textbf{(A)} For the expression $f(x + 2)$ to equal $-1$, we must have $x = -3$.
    Let's verify by substitution:
    \begin{align*}
    f(-1) &= 2(-3)^2 + 7(-3) - 5 \\
    &= 2(9) - 21 - 5 \\
    &= 18 - 21 - 5 = -8
    \end{align*}

\item \textbf{(B)} Let's factor the expression \(a^2x + a^2y - b^2y - b^2x\):
    \begin{align*}
    &= a^2(x + y) - b^2(x + y) \\
    &= (a^2 - b^2)(x + y) \\
    &= (a + b)(a - b)(x + y)
    \end{align*}

\item \textbf{(A)} Given that $x - 1 = 0$ and $x + 1 = 0$ are factors:
    Let $x = 1$ in $x^3 + px^2 + qx + 6 = 0$:
    \begin{align*}
    1 + p + q + 6 &= 0 \\
    p + q &= -7 \quad ...(i)
    \end{align*}
    For $x = -1$:
    \begin{align*}
    -1 + p - q + 6 &= 0 \\
    p - q &= -5 \quad ...(ii)
    \end{align*}
    Solving by elimination:
    \begin{align*}
    2p &= -12 \implies p = -6 \\
    -6 + q &= -7 \implies q = -1
    \end{align*}
    Therefore, $p = -6$ and $q = -1$

\item \textbf{(B)} Using the difference of squares formula:
    \begin{align*}
    \frac{x - 1}{x^2 - 1} &= \frac{x - 1}{(x+1)(x-1)} = \frac{1}{x + 1}
    \end{align*}
    Therefore:
    \begin{align*}
    \frac{1}{x - 1} + \frac{x - 1}{x^2 - 1} &= \frac{1}{x - 1} + \frac{1}{x + 1}
    \end{align*}
    Replacing $x$ with $1-x$:
    \begin{align*}
    \frac{1}{(1-x) - 1} + \frac{1}{(1-x) + 1} &= -\frac{1}{x} + \frac{1}{2-x} \\
    &= -\frac{1}{x} - \frac{1}{x - 2}
    \end{align*}

\item Expand $(x + 3y + 5)(2x^2 + 5y + 2)$:
    \begin{align*}
    &= 2x^3 + 5xy + 2x + 6x^2y + 15y^2 + 6y + 10x^2 + 25y + 10 \\
    &= 2x^3 + 6x^2y + 5xy + 15y^2 + 31y + 10x^2 + 10
    \end{align*}
    \item If $x-1$ divides $kx^3 + 10x^2 + lx - 3$, then $x = 1$ must give zero:
    \begin{align*}
    k(1)^3 + 10(1)^2 + l(1) - 3 &= 0 \\
    k + 10 + l - 3 &= 0 \\
    k + l &= -7 \quad ...(i)
    \end{align*}
    When $x = -2$:
    \begin{align*}
    k(-2)^3 + 10(-2)^2 + l(-2) - 3 &= 27 \
    -8k + 40 - 2l - 3 &= 27 \
    -8k - 2l &= -10 \
    4k + l &= 5 \quad ...(ii)
    \end{align*}
    Solving these equations:
    \begin{align*}
    3k &= 12 \implies k = 4 \
    4 + l &= -7 \implies l = -11
    \end{align*}

    \item \textbf{(E)} Polynomial long division:
        \[
        \begin{array}{r|l}
        & 3x^2 + 7x - 6 \\
        \hline
        x-1 & 3x^3 + 4x^2 - 13x + 6 \\
        \cline{2-2}
        & 3x^3 - 3x^2 \\
        & \underline{\phantom{3x^3} 7x^2 - 13x} \\
        & 7x^2 - 7x \\
        & \underline{\phantom{3x^3 + 7x^2} -6x + 6} \\
        & -6x + 6 \\
        & \underline{\phantom{3x^3 + 7x^2 - 6x +} 0}
        \end{array}
        \]

        Factor \(3x^2 + 7x - 6\):
        \begin{align*}
        3x^2 + 7x - 6 &= 3x^2 + 9x - 2x - 6 \\
        &= 3x(x + 3) - 2(x + 3) \\
        &= (3x - 2)(x + 3)
        \end{align*}
        Therefore, the roots are \((x-1)(x+3)(3x - 2)\).


    \item Factor $(x^2 + x + 1)(x^2 - x + 1)$:
        \begin{align*}
        &= x^4 - x^3 + x^2 + x^3 - x^2 + x + x^2 - x + 1 \
        &= x^4 + x^2 + 1
        \end{align*}
    
    \item 
        \[
        \begin{array}{r|l}
        & x^2 - x - 6 \\
        \hline
        x - 1 & x^3 - 2x^2 - 5x + 6 \\
        \cline{2-2}
        & x^3 - x^2 \\
        & \underline{\phantom{x^3} - x^2 - 5x} \\
        & - x^2 + x \\
        & \underline{\phantom{x^3 - x^2} - 6x + 6} \\
        & - 6x + 6 \\
        & \underline{\phantom{x^3 - x^2 - 6x} 0}
        \end{array}
        \]
        Now solve the quadratic equation:
        \begin{align*}
            x^2 - x - 6 &= x^2 - 3x + 2x - 6 = 0 \\
            &= x(x - 3) + 2(x - 3) = 0 \\
            &= (x + 2)(x - 3) = 0
        \end{align*}
        \[\therefore x = -2 \text{ or } 3\]
        So, its other roots are \(3\) and \(-2\).

    
   \item For \( x - 1 = 0 \), substitute \( x = 1 \):
        \begin{align*}
            lx^3 + 2kx^2 + 24 &= l(1)^3 + 2k(1)^2 + 24 = 0 \\
            &= l + 2k + 24 = 0 \\ 
            &= l + 2k = -24 \hspace{15pt}...(i)
        \end{align*}
        For \( x + 2 = 0 \), substitute \( x = -2 \):
        \begin{align*}
            lx^3 + 2kx^2 + 24 &= l(-2)^3 + 2k(-2)^2 + 24 = 0 \\
            &= -8l + 8k + 24 = 0 \\ 
            &= -8l + 8k = -24 \hspace{15pt}...(ii)
        \end{align*}
        We will solve by elimination to eliminate \( k \). Therefore, we must modify equation (ii) by multiplying by 1:
        \begin{align*}
            -8l + 8k &= -24 \hspace{15pt}...(ii)
        \end{align*}
        So, because the sign of \( k \) in both equations is the same, we will use subtraction:
        \begin{align*} 
                l + 2k &= -24 \hspace{15pt}...(i) \\
            - &\hspace{7pt} -8l + 8k = -24 \hspace{15pt}...(ii) \\
            9l + 10k &= 24
        \end{align*}
        Substitute \( l = -\frac{1}{2} \) into any equation:
        \begin{align*}
            l + 2k = -24 &\Rightarrow -\cfrac{1}{2} + 2k = -24 \\
            k &= -12
        \end{align*}

    \item \textbf{(E)} \( 81a^4 - 16b^4 = \left(9a^2\right)^2 - \left(4b^2\right)^2 \)
        \[\left(9a^2\right)^2 - \left(4b^2\right)^2 = (9a^2 - 4b^2)(9a^2 + 4b^2)\]
        \[ = \left((3a)^2 - (2b)^2\right)(9a^2 + 4b^2)\]
        \[= (3a - 2b)(3a + 2b)(9a^2 + 4b^2)\] 

    \item 
    \[4a^2 - 9b^2 = (2a)^2 - (3b)^2 = (2a - 3b)(2a + 3b)\]
    \[(4a + 6b)^2 = \left(2(2a + 3b)\right)^2 = 2^2 (2a + 3b)^2\]
    \[ 8a^3 + 27b^3 = (2a)^3 + (3b)^3 \]
    To simplify \( (2a)^3 + (3b)^3 \), we should call \( 2a = p \) and \( 3b = q \), and follow along.
    \begin{align*}
        (p + q)^3 &= p^3 + 3p^2q + 3pq^2 + q^3 \\
        &= p^3 + q^3 + 3pq(p + q) \\
        (p + q)^3 - 3pq(p + q) &= p^3 + q^3 \\
        (p + q)((p + q)^2 - 3pq) &= p^3 + q^3
    \end{align*}
    So, let's replace them back:
    \[\Rightarrow (2a)^3 + (3b)^3 = (2a + 3b)\left((2a + 3b)^2 - 3(2a)(3b)\right)\]
    \(\therefore (2a + 3b)\) is common to all 3 expressions.

    \item
    \item \textbf{Advice:} 
    \[ 9 - (x^2 - 3x - 1)^2 = 3^2 - (x^2 - 3x - 1)^2\]  
    \[ = (3 - (x^2 - 3x - 1))(3 + (x^2 - 3x - 1))\]
    \[ = (3 - x^2 + 3x + 1)(3 + x^2 - 3x - 1) \]
    \[= (-x^2 + 3x + 4)(x^2 - 3x + 2)\]
    Let's resolve each part:
    \begin{align*}
    -x^2 + 3x + 4 &= -x^2 - x + 4x + 4 \\
    &= -x(x + 1) + 4(x + 1) \\
    &= (-x + 4)(x + 1)\\
    x^2 - 3x + 2 &= x^2 - x - 2x + 2 \\
    &= x(x - 1) - 2(x - 1) \\
    &= (x - 2)(x - 1)
    \end{align*}
    The factors are \((-x + 4)(x + 1)(x - 2)(x - 1)\).

    \item \textbf{(D)} $f(x - 2) = 4x^2 + x + 7 $ equate $x - 2 = 1 \Rightarrow x = 3$ 
    \begin{align*} 
        f(x - 2) &= 4x^2 + x + 7 \\
        \Rightarrow  f(3 - 2) = f(1) &= 4(3)^2 + 3 + 7 \\
        & = 36 + 10 = 46
    \end{align*}

    \item Replace all \(y\)'s with \(y + 3\)
    \begin{align*} 
        g(y) &= \cfrac{y - 3}{11} + \cfrac{11}{y^2 - 9} \\
       \Rightarrow  g(y + 3) &= \cfrac{(y + 3) - 3}{11} + \cfrac{11}{(y + 3)^2 - 9}  \\
        & = \cfrac{y}{11} + \cfrac{11}{y^2 + 6y + 9 -9} \\
        & = \cfrac{y}{11} + \cfrac{11}{y^2 + 6y} = \cfrac{y}{11} + \cfrac{11}{y(y + 6)}
    \end{align*}
    
    \item 
    \item \textbf{(C)}
        \begin{align*} 
            x^2 + 2a + ax + 2x &= x^2 + ax + 2a + 2x \\
            &= x(x + a) + 2(x + a) \\
            &= (x + 2)(x + a)
        \end{align*}

    \item give
    
    \item Applying the difference of two squares: \(p^2 - q^2 = (p + q)(p - q)\)
        \begin{align*}
            &\Rightarrow [\underbrace{(4a + 3)}_{p} + \underbrace{(3a - 2)}_{q}][\underbrace{(4a + 3)}_{p} - \underbrace{(3a - 2)}_{q}] \\
            &= (7a + 1)(a + 5)
        \end{align*}
    
    \item \textbf{(D)} We should first reduce the equation to its quadratic form:
        \begin{align*}
            & \hspace{5pt} x^2 + 2x - 8 \\
            x - 2 & \overline{x^3 - 12x - 16} \\ 
            - & \hspace{5pt} \underline{x^3 - 2x^2} \\
            & \hspace{30pt} 2x^2 - 12x \\
            - & \hspace{-23pt} \underline{2x^2 - 4x} \\
            & \hspace{55pt} 8x - 16 \\
            - & \hspace{-50pt} \underline{(-8x - 16)}
        \end{align*}
        Factorizing the equation into roots:
        \begin{align*} 
            x^2 + 2x - 8 = 0 &\Rightarrow x^2 + 4x - 2x - 8 = 0 \\
            &= x(x + 4) - 2(x + 4) \\
            &= (x - 2)(x + 4)
        \end{align*}
        Therefore, \(x^3 - 12x - 16 = (x - 2)(x - 2)(x + 4) \) \\
        \(\therefore\) The equation has \(2\) equal roots and a third different root. 
            
    \item \textbf{(D)} For \( x + 1 = 0 \), \(\Rightarrow x = -1\) is a root. \\
        Substituting \( x = -1 \) in the equation \( x^3 - 4x^2 + cx + d \):
        \begin{align*}
            (-1)^3 - 4(-1)^2 + c(-1) + d &= 0 \\
            -1 - 4 - c + d &= 0 \\
            -c + d &= 5
        \end{align*}
        Substituting \( x = -2 \) gives 1:
        \begin{align*}
            (-2)^3 - 4(-2)^2 + c(-2) + d &= 1 \\
            -8 - 16 - 2c + d &= 1 \\
            -2c + d &= 25
        \end{align*}
        Adding the two equations:
        \begin{align*}
            -c + d &= 5 \\
            -(-2c + d) &= -25 \\
            c &= -20
        \end{align*} 
        Substitute \( c = -20 \) in any equation:
        \begin{align*}
            -c + d &= -(-20) + d = 5 \\
            & \Rightarrow \hspace{5pt} d = 5 - 20 = -15
        \end{align*}
        Therefore, \( c = -20 \) and \( d = -15 \). 
    \item 
    
    \item Using the difference of squares: \(p^2 - q^2 = (p + q)(p - q)\)
    \[(x^2 + x)^2 - (2x + 2)^2\]
    \begin{align*}
         &= \left[(x^2 + x) + (2x + 2)\right]\left[(x^2 + x) - (2x + 2)\right] \\
         &= \left[x^2 + x + 2x + 2\right]\left[x^2 + x - 2x - 2\right] \\
         &= \left[x(x + 1) + 2(x + 1)\right]\left[x(x + 1) - 2(x + 1)\right] \\
         &= (x + 1)(x + 1)(x + 2)(x - 2) \\
         &= (x + 1)^2(x + 2)(x - 2)
    \end{align*}
    
    \item Given \(f(x) = 2x^2 + 5x + 3\), replace all \(x\) with \(x + 1\) 
     \begin{align*}
        f(x + 1) &= 2(x + 1)^2+ 5(x +1) + 3 \\
        & = 2(x^2 + 2x + 1) + 5(x + 1) + 3 \\
        & = 2x^2 + 4x + 2 + 5x + 1 + 3 \\
        & = 2x^2 + 9x + 6
     \end{align*}

    \item \textbf{(A)} \begin{align*} 
        & \hspace{5pt} x^ 2 + 2^{-1}x -4^{-1} \\ \vspace{-20pt} 
        x - 2^{-1}& \overline{)x^3 - 8^{-1} \hspace{.5in}} \\
        -\hspace{-1pt} & \hspace{5pt} \underline{x^3 - 2^{-1}x^2} \\
        & \hspace{30pt} 2^{-1}x^2 - 8^{-1} \\
        -\hspace{-25pt} & \hspace{30pt} \underline{2^{-1}x^2 - 4^{-1}x} \\
       -\hspace{-65pt} & \hspace{68pt} 4^{-1}x - 8^{-1} \\
       -\hspace{-65pt} & \hspace{68pt} \underline{4^{-1}x - 8^{-1} } \\
       & \hspace{68pt} \underline{-----} 
    \end{align*}
    The other factor is $x^ 2 + 2^{-1}x -4^{-1}$

    \item \textbf{(D)} Upon careful inspection, we notice that the question allows us to use the difference of squares:
        \[9(x + y)^2 - 4(x - y)^2\]
        Let's make it more useful by setting:
        \[[\underbrace{3(x + y)}_{p}]^2 - [\underbrace{2(x - y)}_{q}]^2\]
        \begin{align*}
            & = \left[3(x + y) - 2(x - y)\right]\left[3(x + y) + 2(x - y)\right] \\
            & = \left(3x + 3y - 2x + 2y\right)\left(3x + 3y + 2x - 2y\right) \\
            & = (x + 5y)(5x - y)
        \end{align*}
    

    \item \textbf{(C)} The first thing to notice is that \(4\) and \(9\) are perfect squares. Additionally, they share factors with \(12\).
        \[4a^2 - 12ab - c^2 + 9b^2 = (2a)^2 - 2 \cdot 2a \cdot 3b - c^2 + (3b)^2\]
        Let \(p = 2a\) and \(q = 3b\),
        \begin{align*}
            &= (2a)^2 - 2 \cdot 2a \cdot 3b - c^2 + (3b)^2 \\
            &= p^2 - 2 \cdot p \cdot q - c^2 + q^2 \\
            &= p^2 - 2pq - c^2 + q^2 \\
            &= p^2 - 2pq + q^2 - c^2 \\
            &= (p - q)^2 - c^2
        \end{align*}
        Applying the difference of squares:
        \begin{align*}
            (p - q)^2 - c^2 &= (p - q - c)(p - q + c)
        \end{align*}
        Replacing them with their initial values:
        \begin{align*}
            (2a - 3b)^2 - c^2 &= (2a - 3b - c)(2a - 3b + c)
        \end{align*}

        \item \textbf{(B)} 
        \begin{align*}
            \frac{1}{2}(3y - 4x)^2 &= \frac{1}{2}(3y - 4x)(3y - 4x) \\
            &= \frac{1}{2}(9y^2 - 12xy - 12xy + 16x^2) \\
            &= \frac{1}{2}(9y^2 - 24xy + 16x^2) \\
            &= \frac{9}{2}y^2 - 12xy + 8x^2 \\ 
            &= 8x^2 - 12xy + \frac{9}{2}y^2 \\ 
            &= 8x^2 + (-12xy) + \frac{9}{2}y^2
        \end{align*}
        By direct comparison, we have:
        \[8x^2 + (-12xy) + \frac{9}{2}y^2 = 8x^2 + kxy + ly^2\]
        Thus, \( k = -12 \) and \( l = \frac{9}{2} \).
        

    \item \textbf{(C)} For \(x - 4 = 2\), \(x = 6\) 
    \begin{align*} 
        f(6 - 4) = f(2) &= 6^2 + 2(6) + 3 \\
        & = 36 + 12 + 3 \\
        & = 51
    \end{align*}

    \item \textbf{(D)} 
        \begin{align*}
            y^3 - 4xy + xy^3 - 4y &= y^3 + xy^3 - 4xy - 4y \\
            &= {y}^{3}(1 + x) - 4y(x + 1) \\
            &= (y^3 - 4y)(x + 1) \\
            &= y(y^2 - 4)(x + 1) \\
            &= y(y - 2)(y + 2)(x + 1) \\
            &= y(x + 1)(y + 2)(y - 2) \\
            &= (y + xy)(y + 2)(y - 2)
        \end{align*}
    
    \item \textbf{(A)} \begin{align*}
        g(x + 1) &= (x + 1) ^2 + 3(x + 1) + 4  \\
        g(x) & = x^2 + 2x + 4 \\
        g(x + 1) - g(x) & = (x+ 1)^2 - x^2 + 3(x+1)  \\
        & \hspace{10pt} - 3x + 4 - 4 \\
        & = (x + 1 - x)(x + 1 + x) \\
        &\hspace{10pt} + 3x + 3 - 3x \\
        & = 2x + 1 + 3 = 2x + 4 = 2(x + 2)
    \end{align*}
    
    \item \textbf{(D)} \begin{align*} 
        m^3 - m -2m^2 + 2 &= m(m^2 -1) -2 (m^2 -1) \\
        & = (m - 2)(m^2 - 1^2) \\
        & = (m-2)(m-1)(m+1)
    \end{align*}

    \item \textbf{(B)} \begin{align*} 
        & = rs -ps + tr - pt \\
        & = s(r-p) + t(r-p) \\
        & = (s + t)(r-p)
    \end{align*}
    $\therefore \hspace{10pt} (r-p) $ is a factor.

    \item \textbf{(A)} If $x + 1$ is a factor, $\therefore$ the value of the $x^3 + 3x^2 + kx + 4 = 0$ when $x = -1$ \\
    \begin{align*}
        x^3 + 3x^2 + kx + 4 &= (-1)^3 + 3(-1)^2 +k(-1) + 4 \\
        & = -1 + 3 -k + 4 = 0 \\
        k & = -6 
    \end{align*}

    \item Notice, \(-q^2\), \(6qr\) and \(-9r^2\) all have a \(q\), \(r\) or both and \(9p^2\) can be expressed as $(3r)^2$, the best i can think of is a difference of two squares. \\
    $$9p^2 - q^2 + 6qr - 9r^2 = (3p)^2 - \underbrace{(9r^2 - 6qr + q^2)}_{\text{like quadratic} }$$ 
    $9r^2 - 6qr + q^2$ can be expressed without $q$,  $9r^2 - 6r + 1$ 
    \begin{align*}
    9r^2 - 6r + 1 &= 9r^2 - 3r - 3r + 1 \\
    &= 3r(3r -1) -(3r -1) \\ 
    &= (3r -1)^2 \\
    9r^2 - 6qr + q^2  &= (3r -q)^2 \\
    9p^2 - q^2 + 6qr - 9r^2 &= (3p)^2 - (3r -q)^2 \\
    &= (3p + 3r - q)(3p - 3r + q) 
    \end{align*}

    \item \textbf{(B)} $x+1 = 0$ when $x = -1$ 
    \begin{align*} 
        f(0) = f(-1 + 1) &= 3(-1)^2 - (-1) + 4 \\
        & = 3 + 1 + 4 = 8
    \end{align*}

    \item $x+2 = 1$ at $x = -1$ 
    \begin{align*} 
        f(1) = f(-1 + 2) &= 3(-1)^2 + 4(-1) + 1 \\
        & = 3 - 4 + 1 = 0
    \end{align*}

    \item \textbf{(B)} they all share factors with 2 
     \begin{align*} 
        2(3x^2 - 7x - 6) & = 2(3x^2 - 9x + 2x -6) \\
        & = 2\left(3x(x - 3) + 2(x - 3)\right) \\
        & = 2(x-3)(3x +2)
    \end{align*}
    
    \item \textbf{(A)} $abx^2 -4bx -2axy + 8y$  \\
    $= bx(ax - 4) - 2y(ax - 4)$ \\
    $=(ax -4)(bx-2y)$

    \item \textbf{(C)} $1^2 - (a -b)^2 = (1 +a -b)(1 -a + b)$

    \item\textbf{(B)} \begin{align*}
        -2x^2 + 7x + 15 &= -2x^2 + 10x - 3x + 15 \\
        & = -2x(x -5) -3(x-5) \\
        & = (-2x -3)\underbrace{(x-5)}_{factor}
    \end{align*}
    
    \item \textbf{(A)} I'd like to take a different approach for this problem rather than long division \\
    \begin{align*} 
        \cfrac{x^3 - x  + 7x^2 - 7}{x^2 - 1} & = \cfrac{x(x^2 -1) + 7(x^2 -1)}{x^2 - 1}  \\
        & = \cfrac{(x+7)(\cancel{x^2 - 1})}{\cancel{x^2 -1}} = x+7
    \end{align*}
    \item if $x-p$ leaves remainder of 6  \\
    $2(p)^2 -p(p) + p = 6 \hspace{7pt} \Rightarrow  \underbrace{p}_{2} \underbrace{(p+1)}_{3} = 6$ \\
    $\therefore \hspace{10pt} p = 2$
    \item when divided by $(m-1)$ the remainder is $2$ \\
    $\therefore p(1)^2 + q(1) + 1 = 2 \text{ and } p + q = 1$\\
    when divided by $(m+1)$, remainder is $4$ \\
    $p(-1)^2 + q(-1) = p -q = 4$
    \begin{align*} 
        p + q &= 2 \hspace{20pt} ...(i) \\
       +\hspace{5pt}  p - q &= 4 \hspace{20pt} ...(ii) \\
       2p & = 6, \hspace{10pt} p = 3, q = -1
    \end{align*}
\item \textbf{(A)} 
    \(r^2 - 2pr - rq + 2pq = r^2 - rq - 2pr + 2pq \)\\
    \(= r(r - q) - 2p(r - q) = (r - q)(r - 2p)\)    
\item \textbf{(A)} 
        \begin{align*}
            & \hspace{5pt} x^2 + 5x + 6 \\
            2x + 1 \hspace{5pt} & \overline{) \hspace{3pt} 2x^3 + 11x^2 + 17x + 6} \\
            - & \hspace{5pt} \underline{2x^3 + x^2} \\
            & \hspace{30pt} 10x^2 + 17x \\
            - \hspace{-25pt} & \hspace{30pt} \underline{10x^2 + 5x} \\
            & \hspace{63pt} 12x + 6 \\
            - \hspace{-60pt} & \hspace{63pt} \underline{12x + 6} \\
            & \hspace{63pt} \underline{----}
        \end{align*}    
\item \textbf{(A)} \( x^2 + 2xy + y^2 = (x+y)^2 \) \\
    \( (x+y)^2 + 3(x+y) - 18 = 0 \) let \( x+y = k \) 
    \begin{align*}
    k^2 + 3k - 18 &= k^2 + 6k - 3k - 18 \\
    &= k(k+6) - 3(k+6) \\
    &= (k+6)(k-3)
    \end{align*}
    replace \( k \) back \( (x+y+6)(x+y-3) \)
\item 
    \begin{align*}
        & 2x^2 + x - 1  \\
        2x - 1 \hspace{5pt} & \overline{)\hspace{3pt} 4x^3 - 3x + 1} \\
        -\hspace{-2pt} & \hspace{8pt} \underline{4x^3 - 2x^2} \\
        & \hspace{36pt} 2x^2 - 3x \\
        -\hspace{-30pt} & \hspace{36pt} \underline{2x^2 - x} \\
        & \hspace{51pt} {-2x + 1} \\
        -\hspace{-45pt} & \hspace{51pt} \underline{-2x + 1} \\
        & \hspace{51pt} \underline{----}
    \end{align*}
\item
\item \textbf{(B)} \( -9y^2 = -(3y)^2 \) carries the negative sign, so this is a difference of two squares problem. We would rearrange
        \[(4x^2 + 20x + 25) - 9y^2 \]
        Producing a square for the left-hand side
        \begin{align*}
        &4x^2 + 20x + 25 
        &= 4x^2 + 10x + 10x + 25 \\
        &= 2x(2x + 5) + 5(2x + 5) \\
        &= (2x + 5)^2
        \end{align*}
    \[(2x + 5)^2 - (3y)^2 = (2x + 5 - 3y)(2x + 5 + 3y) \] 
\item \textbf{(B)} To avoid difficulties let \( a^x = p \) \\
    now divide \( p^3 - 26p^2 + 156p - 216 \) by \( p^2 - 24p + 108 \):
    \begin{align*} 
        & \hspace{8pt} p - 2 \\
        p^2 - 24p + 108 \hspace{5pt} & \overline{)\hspace{3pt} p^3 - 26p^2 + 156p - 216} \\
       -\hspace{-1pt} & \hspace{7pt} \underline{p^3 - 24p^2 + 108p} \\
       & \hspace{25pt} {-2p^2 + 48p - 216} \\
      -\hspace{-20pt} & \hspace{25pt} \underline{-2p^2 + 48p - 216} \\
      & \hspace{25pt} \underline{--------}
    \end{align*}
    The result is \( p - 2 = a^x - 2 \)
\item
\item \textbf{(A)} \( x = \cfrac{4}{3} \) and \( x = -\cfrac{3}{5} \), \hspace{5pt} \( \therefore  x-\cfrac{4}{3} = 0 \) and \( x+\cfrac{3}{5} = 0 \) 
    \begin{align*}
    \left(x-\cfrac{4}{3}\right)\left(x+\cfrac{3}{5}\right) &= x^2 + \cfrac{3}{5}x - \cfrac{4}{3}x + \left(-\cfrac{4}{3} \times \cfrac{3}{5}\right) \\
    &= x^2  +  \cfrac{9 - 20}{15}\,x -\cfrac{4}{5} \\
    &= x^2 - \cfrac{11}{15}\,x -\cfrac{4}{5} \\
    &= 15x^2 - 11x - 12 = 0
    \end{align*}
\item 
    \begin{align*}
    &\hspace{6pt} 3x - 2y \\
        9x^2 + 6xy + 4y^2 \hspace{5pt}  & \overline{\hspace{2pt} 27x^3 - 8y^3 \hspace{1in}} \\
      -\hspace{-3pt} & \hspace{6pt} \underline{27x^3 + 18x^2y + 12xy^2} \\
      & \hspace{32pt} {-18x^2y - 12xy^2 - 8y^3} \\
     -\hspace{-26pt} & \hspace{32pt} \underline{-18x^2y - 12xy^2 -8y^3}\\
     & \hspace{32pt} \underline{----------}
    \end{align*}
    The other factor is \(3x - 2y\)
\item 
    \begin{align*}
    &\hspace{6pt} 3x - 2y \\
        9x^2 + 6xy + 4y^2 \hspace{5pt}  & \overline{\hspace{2pt} 27x^3 - 8y^3 \hspace{1in}} \\
      -\hspace{-3pt} & \hspace{6pt} \underline{27x^3 + 18x^2y + 12xy^2} \\
      & \hspace{32pt} {-18x^2y - 12xy^2 - 8y^3} \\
     -\hspace{-26pt} & \hspace{32pt} \underline{-18x^2y - 12xy^2 -8y^3}\\
     & \hspace{32pt} \underline{----------}
    \end{align*}
    The other factor is $3x - 2y$
\item \textbf{(C)} \\
    \[\cfrac{x(x^2 + 3x - 10)}{2(x^2 - 4)} = \cfrac{x\cancel{(x-2)}(x+5)}{2\cancel{(x-2)}(x+2)} = \cfrac{x(x+5)}{2(x+2)}\]
        \begin{align*}
        x^2 + 3x - 10 &= x^2 + 5x - 2x - 10 \\ 
        &= x(x+5) - 2(x+5) \\ 
        &= (x-2)(x+5) \\
        x^2 - 4 &= x^2 - 2^2 \\ 
        &= (x-2)(x+2)
        \end{align*}    
\item 
\item for $x+3 = 0 , x = -3$, subsitute $x=-3$ into the polynomial \\
    $$3(-3)^3 + 5(-3)^2 + 11(-3) - 4 = -81 + 45 -33 - 4$$ 
    \item \textbf{(B)} solve it without one of the variable, i'd work without $x$ 
    \begin{align*}
    2y^2 - 15y + 18 &= 2y^2 -12y - 3y + 18  \\ 
    &= 2y(y-6) -3(y-6)  \\ 
    &= (2y-3)(y-6)
    \end{align*}
    Replace the $x$ on those without any variable 
    $$(2y-3x)(y-6x)$$
    \item if $y-1$ is a factor then $1$ is a root 
    \begin{align*}
    1^3 + 4(1)^2 + k(1) - 6 &= 0 \\
    3+ 4 + k - 6 &= 0 \\
    k & = -1
    \end{align*}
    \item \textbf{(B)} 
    \begin{align*} 6x^2 + 3x + 10x + 5 &= 3x(2x + 1) + 5(2x+1) \\ &= (3x+5)(2x+1) \end{align*}
    \item \textbf{(C)} if $-2, -1 \text{ and } 3$ are roots, then $(x+2), (x+1) \text{ and } (x-3)$ are factors 
        \begin{align*} 
            (x+2)(x+1)(x-3) &= 0 \\
            (x^2 + 2x + x + 2)(x-3) &= 0 \\
            (x^2 + 3x + 2)(x-3) &= 0 \\
            x^3 - 3x^2 +3x^2 - 9x + 2x -6 & = 0 \\
            x^3 -7x -6 & = 0 
        \end{align*}
    \item for $2x+1 = 0, x = -\cfrac{1}{2}$ \\
    \begin{align*} 
        k(-\cfrac{1}{2})^3 + 
    \end{align*}
    \item
    \item
    \item 
    \item 
    \item 
    \item 
    \item
    \item
    \item
    \item 
    \item
    \item
    \item 
    \item 
    \item 
    \item 
    \item
    \item
    \item
    \item 
    \item
    \item
    \item 
    \item 
    \item 
    \item 
    \item
    \item
    \item
    \item 
    \item
    \item
    \item 
    \item 
\end{enumerate}
\end{multicols}