\chapter{Algebra}
\section{Factorization and Remainder Theorem}
\subsection{Questions}
\begin{multicols}{2}
\begin{enumerate}[label={\arabic*.}]
\item If the function \(f\) is defined by \(f(x+2)\) = \(2{x}^{2} + 7x -5\), find \(f(-1)\)
	\begin{enumerate}[label={\Alph*.}]
	\item \(-8\)
	\item \(4\)
	\item \(10\)
	\item \(-10\)
	\end{enumerate}
\item Factorize \(a^2x - b^2y - b^2x + a^2y\)
	\begin{enumerate}[label={\Alph*.}]
	\item \((y-x)(a-b)(a+b)\)
	\item \((a-b)(x+y)\)
	\item \((x-y)(a-b)\)
	\item \((x+y)(a-b)(a+b)\)
	\end{enumerate}
\item if \(x - 1\) and \(x + 1\) are both factors of the equation: \({x}^{3} + p{x}^{2} + qx + 6 \) = 0, 
evaluate $p$ and $q$
	\begin{enumerate}[label={\Alph*.}]
	\item \(-6, -1\)
	\item \(1, -1\)
	\item \(6, 1\)
	\item \(6, -6\)
	\end{enumerate}
\item if \(f(x)\) = \(\dfrac{1}{x - 1} + \dfrac{x - 1}{{x}^{2} - 1}\), find \(f(1 - x)\)
	\begin{enumerate}[label={\Alph*.}]
	\item \(\dfrac{1}{x} + \dfrac{1}{x - 2}\)
	\item \( -\dfrac{1}{x} - \dfrac{1}{x - 2}\)
	\item \(x + \dfrac{1}{2x - 1}\)
	\item \(\dfrac{1}{x} + \dfrac{1}{{x}^{2} - 1}\)
	\item \(-\dfrac{1}{x} - \dfrac{1}{2x - 1}\)
	\end{enumerate}
\item Multiply (\(x + 3y + 5\)) by (\(2{x}^{2} + 5y + 2\))
	\begin{enumerate}[label={\Alph*.}]
	\item \(2{x}^{3} + 3{x}^{2}y + 10xy^2 + 13y + 10{x}^{2} + 2x + 10\)
	\item \(2{x}^{3} + 2{x}^{2}y + 10xy + 10y^2 +  31y + 5{x}^{2} + 2x + 10\)
	\item \(2{x}^{3} + 6{x}^{2}y + 5xy + 10y^2 + 13y + 5{x}^{2} + 2x + 10\)
	\item \(2{x}^{3} + 6{x}^{2}y + 5xy + 15y^2 + 31y + 5{x}^{2} + 2x + 10\)
	\item \(2{x}^{3} + 3{x}^{2}y + 5xy + 10y^2 + 13y + 5{x}^{2} + 2x + 10\)
	\end{enumerate}
\item If \(k{x}^{3} + 	10{x}^{2} + lx - 3\) is divisible by (\(x - 1\)) and if when it is divided by (\(x + 2\)) the remainder is 27,
find the constant \(k\) and \(l\).
	\begin{enumerate}[label={\Alph*.}]
	\item \(k = -7, l = -15\)
	\item \(k = \cfrac{-21}{5}, l = \cfrac{-61}{5}\)
	\item \(k =-15, l =-7\)
	\item \(k = -\cfrac{5}{3}, l = \cfrac{19}{5}\)
	\item \(k = -\cfrac{5}{3}, l = -\cfrac{19}{3}\)
	\end{enumerate}
\item Factorize \(3{x}^{3} + 4{x}^{2} - 13x + 6\) completely, given that \(x - 1\) is a factor
	\begin{enumerate}[label={\Alph*.}]
	\item \((x-1)(x-3)(x+2)\)
	\item \((x-1)(x-3)(3x+2)\)
	\item \((x-1)(x-2)(x+3)\)
	\item \((x-1)(x+3)(3x+2)\)
	\item \((x-1)(x+3)(3x-2)\)
	\end{enumerate}
\item Multiply \({x}^{2}+x+1\) by \({x}^{2}-x+1\)
	\begin{enumerate}[label={\Alph*.}]
	\item \(x^4+3{x}^{2}+x+1\)
	\item \(x^4+4{x}^{2}-6x+1\)
	\item \(x^4+4{x}^{2}+1\)
	\item \(x^4-{x}^{3}-{x}^{2}+x+1\)
	\item \(x^4-6{x}^{2}-4x+1\)
	\end{enumerate}
\item If \(x=1\) is a root of the equation: \({x}^{3}-2{x}^{2}-5x+6\), find the other roots.
	\begin{enumerate}[label={\Alph*.}]
	\item -3 and 2
	\item 1 and 3
	\item -2 and 2
	\item 3 and -2
	\item -3 and 1
	\end{enumerate}
\item If \(x+2\) and \(x-1\) are factors of the expression: \(l{x}^{3}+2k{x}^{2}+24\), find the values of \(l\) and \(k\)
	\begin{enumerate}[label={\Alph*.}]
	\item \(l=-6, k=-9\)
	\item \(l=-2, k=-1\)
	\item \(l=-2, k=1\)
	\item \(l=0, k=1\)
	\item \(l=6, k=0\)
	\end{enumerate}
\item Factorize completely: \(81a^4-16b^4\)
	\begin{enumerate}[label={\Alph*.}]
	\item \((3a+2b)(2a-3b)(9a^2+4b^2)\)
	\item \((3a-2b)(2a-3b)(9a^2-4b^2)\)
	\item \((3a-2b)(3a-2b)(9a^2+4b^2)\)
	\item \((3a-2b)(2a-3b)(4a^2-9b^2)\)
	\item \((3a-2b)(3a+2b)(9a^2+4b^2)\)
	\end{enumerate}
\item The factor which is common to all three bionomial expressions: \(4a^2-9b^2\), \(8a^2+27b^3\), \((4a+6b)^2\)
	\begin{enumerate}[label={\Alph*.}]
	\item \(4a-6b\)
	\item \(4a+6b\)
	\item \(2a-3b\)
	\item \(2a+3b\)
	\item \(3a-2b\)
	\end{enumerate}
\item If \(x-2\) and \(x+1\) are factors of the expression: \({x}^{3}+p{x}^{2}+qx+1\)
	\begin{enumerate}[label={\Alph*.}]
	\item \(-3\)
	\item \(0\)
	\item \(-\dfrac{17}{3}\)
	\item \(-\dfrac{2}{3}\)
	\item \(3\)
	\end{enumerate}
\item The factors of \(9-({x}^{2}-3x-1)^2\) are. 
	\begin{enumerate}[label={\Alph*.}]
	\item \((x-4)(x-1)(x-1)(x+2)\)
	\item \((x-4)(x+1)(x-2)(x-1)\)
	\item \((x-2)(x+2)(x+1)(x+4)\)
	\item \((x-2)(x+2)(x+1)(x-1)\)
	\item \((x-4)(x-3)(x-2)(x+1)\)
	\end{enumerate}
\item If \(f(x-2) = 4{x}^{2} + x + 7 \) find \(f(1)\)
	\begin{enumerate}[label={\Alph*.}]
	\item \(27\)
	\item \(7\)
	\item \(17\)
	\item \(46\)
	\item \(12\)
	\end{enumerate}
\item If \(g(y) = \dfrac{y - 3}{11} + \dfrac{11}{y^2-9}\) what is \(g(y+3)\)
	\begin{enumerate}[label={\Alph*.}]
	\item \(\dfrac{y}{11} + \dfrac{11}{y(y+5)}\)
	\item \(\dfrac{y+30}{11} + \dfrac{11}{y(y+3)}\)
	\item \(\dfrac{y}{11} + \dfrac{11}{y(y+3)}\)
	\item \(\dfrac{y+3}{11}+\dfrac{11}{y(y-6)}\)
	\end{enumerate}
\item Factorize completely \(3a+125a^3\)
	\begin{enumerate}[label={\Alph*.}]
	\item \((2a+5x)(4+10ax + 25a{x}^{2})\)
	\item \((2a+5{x}^{2})(4+25ax)\)
	\item \(a(2+5x)(4-10x+25a{x}^{2})\)
	\item \(a(2+5x)(4+10ax+25a{x}^{2})\)
	\end{enumerate}
\item Factorize \({x}^{2}+2a+ax+2x\)
	\begin{enumerate}[label={\Alph*.}]
	\item \(({x}^{2}-1)(x+a)\)
	\item \((x+2)(x+a)\)
	\item \((x+2a)(x+3)\)
	\item \((x+2a)(x-1)\)
	\end{enumerate}
\item The graphical method of solving the equation: \({x}^{3}+3{x}^{2}+4x-28 = 0\) is by drawing the graphs of the curves
	\begin{enumerate}[label={\Alph*.}]
	\item \(y = {x}^{3}\) and \(y=3{x}^{2} + x -28\)
	\item \(y={x}^{3}+3{x}^{2}+4x\) and \(y\)
	\item \(y={x}^{3}+3{x}^{2}+4x-28\) and the line \(y=\dfrac{28}{x}\)
	\item \(y={x}^{2}+3x+4\) and \(y=\dfrac{28}{x}\)
	\item \(y={x}^{2}+3x+4\) and line \(y=28x\)
	\end{enumerate}
\item Factorize \((4a+3)^2-(3a-2)^2\)
	\begin{enumerate}[label={\Alph*.}]
	\item \((x+2a)(x-1)\)
	\item \((x+1)(x+2a)\)
	\item \((x+2)(x+a)\)
	\item \(({x}^{2}-1)(x+a)\)
	\end{enumerate}
\item If \({x}^{3} - 12x - 16 = 0\) has \(x-2\) as a solution, then the equation has
	\begin{enumerate}[label={\Alph*.}]
	\item 3 roots all different
	\item \(x-4\) as a solution also
	\item 3 roots all equal
	\item 3 roots with two equal and the third different
	\item only one root
	\end{enumerate}
\item The expression: \({x}^{3}-4{x}^{2}+cx+d\) is such that \(x+1\) is a factor and its values is 1 when x is -2. find \(c\) and \(d\)
	\begin{enumerate}[label={\Alph*.}]
	\item \(c=-4\) and \(d=9\)
	\item \(c=20\) and \(d =9\)
	\item \(c=-20\) and \(d=15\)
	\item \(c=-20\) and \(d=-15\)
	\item \(c=20\) and \(d=-15\)
	\end{enumerate}
\item What factor is common to all the expressions: \(x+1, 2{x}^{2}+x+1\) and \({x}^{2}-1\)
	\begin{enumerate}[label={\Alph*.}]
	\item \(x+1\)
	\item \(1\)
	\item No common factor
	\item \(2x-1\)
	\item \(x\)
	\end{enumerate}
\item \textbf{(B)} Facorize completely: \(({x}^{2}+x)^2-(2x+2)^2\)
	\begin{enumerate}[label={\Alph*.}]
	\item \((x+y)(x+2)(x-2)\)
	\item \((x+1)^2(x+2)(x-2)\)
	\item \((x+y)^2(y-2)^2\)
	\item \((x+1)^2(x+2)^2\)
	\end{enumerate}
\item if \(f(x) = 2{x}^{2}+5x+3\), find \(f(x+1)\)
	\begin{enumerate}[label={\Alph*.}]
	\item \(2{x}^{2}-x+10\)
	\item \(2{x}^{2}-x\)
	\item \(4{x}^{2}+3x+12\)
	\item \(4{x}^{2}+3x+2\)
	\end{enumerate}
\item If one factor of \({x}^{3}-8^{-1}\) is \(x-2^{-1}\), the other factor is
	\begin{enumerate}[label={\Alph*.}]
	\item \({x}^{2}+2^{-1}x-4^{-1}\)
	\item \({x}^{2}-2^{-1}x-4^{-1}\)
	\item \({x}^{2}-2^{-1}x-4^{-1}\)
	\item \({x}^{2}+4^{-1}x-2^{-1}\)
	\end{enumerate}
\item Factorize \(9(x+y)^2 - 4(x-y)^2\)
	\begin{enumerate}[label={\Alph*.}]
	\item \((x+y)(5x+y)\)
	\item \((x+y)^2\)
	\item \(5(x+y)^2\)
	\item \((x+5y)(5x-y)\)
	\end{enumerate}
\item Factorize \(4a^2-12ab-c^2+9b^2\)
	\begin{enumerate}[label={\Alph*.}]
	\item \((2a+3b-c)(2a+3b+c)\)
	\item \(4a(a-3b)+(3b-c)^2\)
	\item \((2a-3b-c)(2a-3b+c)\)
	\item \(4a(a-3b) + (3b+c)^2\)
	\end{enumerate}
\item What are \(k\) and \(l\) respectively if: \(\dfrac{1}{2}(3y-4x)^2 = (8{x}^{2}+kxy+ly^2)\)
	\begin{enumerate}[label={\Alph*.}]
	\item \(12, \dfrac{9}{2}\)
	\item \(-12, \dfrac{9}{2}\)
	\item \(6, 9\)
	\item \(-6, 9\)
	\end{enumerate}
\item if \(f(x-4) = {x}^{2}+2x+3\), find \(f(2)\)
	\begin{enumerate}[label={\Alph*.}]
	\item \(11\)
	\item \(6\)
	\item \(51\)
	\item \(27\)
	\end{enumerate}
\item Factorize completely: \(y^3-4xy+xy^3-4y\)
	\begin{enumerate}[label={\Alph*.}]
	\item \(y(1-x)(y+2)(y-2)\)
	\item \(y(1+x)(y-2)(y-2)\)
	\item \((y+xy)(y+2)(y-2)\)
	\item \((y+xy)(y+2)(y-2)\)
	\end{enumerate}
\item If \(g(x) = {x}^{2}+3x+4, find g(x+1) -g(x)\)
	\begin{enumerate}[label={\Alph*.}]
	\item \(2(x+2)\)
	\item \((x+2)\)
	\item \((2x+1)\)
	\item \({x}^{2}+4\)
	\end{enumerate}
\item Factorize: \(m^3-2m^2-m+2\)
	\begin{enumerate}[label={\Alph*.}]
	\item \((m+1)(m+1)(m+2)\)
	\item \((m^2+1)(m-2)\)
	\item \((m^2+2)(m-1)\)
	\item \((m-2)(m+1)(m-1)\)
	\end{enumerate}
\item Which of the following is a factor of \(rs+tr-pt-ps\)
	\begin{enumerate}[label={\Alph*.}]
	\item \((p-s)\)
	\item \((r-p)\)
	\item \((s-p)\)
	\item \((r+p)\)
	\end{enumerate}
\item If \(x+1\) is a factor of: \({x}^{3}+3{x}^{2}+kx+4\), find the value of k
	\begin{enumerate}[label={\Alph*.}]
	\item \(-6\)
	\item \(6\)
	\item \(8\)
	\item \(-8\)
	\end{enumerate}
\item Factorize: \(9p^2-q^2+6pr-9r^2\)
	\begin{enumerate}[label={\Alph*.}]
	\item \((3p-3q+r)(3p-q)\)
	\item \((6p-3q-3r)(3p-q-4r)\)
	\item \((3p-3q+r)(3p-q-3r)\)
	\item \(\)
	\end{enumerate}
\item if a function is defined by $f(x+1) = 3x^2-x+4$, find $f(0)$
	\begin{enumerate}[label={\Alph*.}]
	\item \(6\)
	\item \(8\)
	\item \(0\)
	\item \(2\)
	\item \(4\)
	\end{enumerate}
\item $f(x+2) = 3x^2 + 4x + 1$. find $f(1)$
	\begin{enumerate}[label={\Alph*.}]
	\item \(32\)
	\item \(40\)
	\item \(8\)
	\item \(32\)
	\item \(21\)
	\end{enumerate}
\item Factorize: $6x^2 -14x - 12$
	\begin{enumerate}[label={\Alph*.}]
	\item \(2(x+3)(3x-2)\)
	\item \(2(x-3)(3x +2)\)
	\item \(6(x-2)(x+1)\)
	\item \(6(x+2)(x-1)\)
	\item \((3x+4)(2x+3)\)
	\end{enumerate}
\item Factorize: $abx^2 - 8y -4bx - 2axy$
	\begin{enumerate}[label={\Alph*.}]
	\item \((ax -4)(bx-2y)\)
	\item \((bx-4)(ax-2y)\)
	\item \((ax+b)(x-8y)\)
	\item \((x-2y)(abx-4)\)
	\item \((ax-2y)(by-4)\)
	\end{enumerate}
\item Factorize: $ 1- (a-b)^2$
	\begin{enumerate}[label={\Alph*.}]
	\item \((1 +a+b)(1-a-b)\)
	\item \((1-a + b)(1+ a -b)\)
	\item \((1 + a - b)(1-a+b)\)
	\item \((1 -a -b)(1-a + b)\)
	\item \((1 -a +b)(1+a + b)\)
	\end{enumerate}
\item Which of the following is a factor of: $15 + 7x -2x^2$
	\begin{enumerate}[label={\Alph*.}]
	\item \(x +3\)
	\item \(x-5\)
	\item \(x+5\)
	\item \(x-3\)
	\end{enumerate}
\item Divide the expression: $x^3 + 7x^2 -x -7$ by $-1 + x^2$
	\begin{enumerate}[label={\Alph*.}]
	\item \(x+1\)
	\item \(-x^3 + 7x^2 -x -7\)
	\item \(x-7\)
	\item \(-x^2 + 7x + 7\)
	\end{enumerate}
\item
	\begin{enumerate}[label={\Alph*.}]
	\item \(\)
	\item \(\)
	\item \(\)
	\item \(\)
	\end{enumerate}
\item
	\begin{enumerate}[label={\Alph*.}]
	\item \(\)
	\item \(\)
	\item \(\)
	\item \(\)
	\end{enumerate}
\item
	\begin{enumerate}[label={\Alph*.}]
	\item \(\)
	\item \(\)
	\item \(\)
	\item \(\)
	\end{enumerate}
\item
	\begin{enumerate}[label={\Alph*.}]
	\item \(\)
	\item \(\)
	\item \(\)
	\item \(\)
	\end{enumerate}
\item
	\begin{enumerate}[label={\Alph*.}]
	\item \(\)
	\item \(\)
	\item \(\)
	\item \(\)
	\end{enumerate}
\item
	\begin{enumerate}[label={\Alph*.}]
	\item \(\)
	\item \(\)
	\item \(\)
	\item \(\)
	\end{enumerate}
\item
	\begin{enumerate}[label={\Alph*.}]
	\item \(\)
	\item \(\)
	\item \(\)
	\item \(\)
	\end{enumerate}
\item
	\begin{enumerate}[label={\Alph*.}]
	\item \(\)
	\item \(\)
	\item \(\)
	\item \(\)
	\end{enumerate}
\item
	\begin{enumerate}[label={\Alph*.}]
	\item \(\)
	\item \(\)
	\item \(\)
	\item \(\)
	\end{enumerate}
\item
	\begin{enumerate}[label={\Alph*.}]
	\item \(\)
	\item \(\)
	\item \(\)
	\item \(\)
	\end{enumerate}
\item
	\begin{enumerate}[label={\Alph*.}]
	\item \(\)
	\item \(\)
	\item \(\)
	\item \(\)
	\end{enumerate}
\item
	\begin{enumerate}[label={\Alph*.}]
	\item \(\)
	\item \(\)
	\item \(\)
	\item \(\)
	\end{enumerate}
\item
	\begin{enumerate}[label={\Alph*.}]
	\item \(\)
	\item \(\)
	\item \(\)
	\item \(\)
	\end{enumerate}
\item
	\begin{enumerate}[label={\Alph*.}]
	\item \(\)
	\item \(\)
	\item \(\)
	\item \(\)
	\end{enumerate}
\item
	\begin{enumerate}[label={\Alph*.}]
	\item \(\)
	\item \(\)
	\item \(\)
	\item \(\)
	\end{enumerate}
\item
	\begin{enumerate}[label={\Alph*.}]
	\item \(\)
	\item \(\)
	\item \(\)
	\item \(\)
	\end{enumerate}
\item
	\begin{enumerate}[label={\Alph*.}]
	\item \(\)
	\item \(\)
	\item \(\)
	\item \(\)
	\end{enumerate}
\item
	\begin{enumerate}[label={\Alph*.}]
	\item \(\)
	\item \(\)
	\item \(\)
	\item \(\)
	\end{enumerate}
\item
	\begin{enumerate}[label={\Alph*.}]
	\item \(\)
	\item \(\)
	\item \(\)
	\item \(\)
	\end{enumerate}
\item
	\begin{enumerate}[label={\Alph*.}]
	\item \(\)
	\item \(\)
	\item \(\)
	\item \(\)
	\end{enumerate}
\item
	\begin{enumerate}[label={\Alph*.}]
	\item \(\)
	\item \(\)
	\item \(\)
	\item \(\)
	\end{enumerate}
\item
	\begin{enumerate}[label={\Alph*.}]
	\item \(\)
	\item \(\)
	\item \(\)
	\item \(\)
	\end{enumerate}
\item
	\begin{enumerate}[label={\Alph*.}]
	\item \(\)
	\item \(\)
	\item \(\)
	\item \(\)
	\end{enumerate}
\item
	\begin{enumerate}[label={\Alph*.}]
	\item \(\)
	\item \(\)
	\item \(\)
	\item \(\)
	\end{enumerate}
\item
	\begin{enumerate}[label={\Alph*.}]
	\item \(\)
	\item \(\)
	\item \(\)
	\item \(\)
	\end{enumerate}
\item
	\begin{enumerate}[label={\Alph*.}]
	\item \(\)
	\item \(\)
	\item \(\)
	\item \(\)
	\end{enumerate}
\item
	\begin{enumerate}[label={\Alph*.}]
	\item \(\)
	\item \(\)
	\item \(\)
	\item \(\)
	\end{enumerate}
\item
	\begin{enumerate}[label={\Alph*.}]
	\item \(\)
	\item \(\)
	\item \(\)
	\item \(\)
	\end{enumerate}
\item
	\begin{enumerate}[label={\Alph*.}]
	\item \(\)
	\item \(\)
	\item \(\)
	\item \(\)
	\end{enumerate}
\item
	\begin{enumerate}[label={\Alph*.}]
	\item \(\)
	\item \(\)
	\item \(\)
	\item \(\)
	\end{enumerate}
\item
	\begin{enumerate}[label={\Alph*.}]
	\item \(\)
	\item \(\)
	\item \(\)
	\item \(\)
	\end{enumerate}


\item
	\begin{enumerate}[label={\Alph*.}]
	\item \(\)
	\item \(\)
	\item \(\)
	\item \(\)
	\end{enumerate}
\item
	\begin{enumerate}[label={\Alph*.}]
	\item \(\)
	\item \(\)
	\item \(\)
	\item \(\)
	\end{enumerate}
\item
	\begin{enumerate}[label={\Alph*.}]
	\item \(\)
	\item \(\)
	\item \(\)
	\item \(\)
	\end{enumerate}
\item
	\begin{enumerate}[label={\Alph*.}]
	\item \(\)
	\item \(\)
	\item \(\)
	\item \(\)
	\end{enumerate}
\item
	\begin{enumerate}[label={\Alph*.}]
	\item \(\)
	\item \(\)
	\item \(\)
	\item \(\)
	\end{enumerate}
\item
	\begin{enumerate}[label={\Alph*.}]
	\item \(\)
	\item \(\)
	\item \(\)
	\item \(\)
	\end{enumerate}
\item
	\begin{enumerate}[label={\Alph*.}]
	\item \(\)
	\item \(\)
	\item \(\)
	\item \(\)
	\end{enumerate}
\item
	\begin{enumerate}[label={\Alph*.}]
	\item \(\)
	\item \(\)
	\item \(\)
	\item \(\)
	\end{enumerate}
\item
	\begin{enumerate}[label={\Alph*.}]
	\item \(\)
	\item \(\)
	\item \(\)
	\item \(\)
	\end{enumerate}
\item
	\begin{enumerate}[label={\Alph*.}]
	\item \(\)
	\item \(\)
	\item \(\)
	\item \(\)
	\end{enumerate}
\item
	\begin{enumerate}[label={\Alph*.}]
	\item \(\)
	\item \(\)
	\item \(\)
	\item \(\)
	\end{enumerate}
\item
	\begin{enumerate}[label={\Alph*.}]
	\item \(\)
	\item \(\)
	\item \(\)
	\item \(\)
	\end{enumerate}
\item
	\begin{enumerate}[label={\Alph*.}]
	\item \(\)
	\item \(\)
	\item \(\)
	\item \(\)
	\end{enumerate}
\item
	\begin{enumerate}[label={\Alph*.}]
	\item \(\)
	\item \(\)
	\item \(\)
	\item \(\)
	\end{enumerate}
\item
	\begin{enumerate}[label={\Alph*.}]
	\item \(\)
	\item \(\)
	\item \(\)
	\item \(\)
	\end{enumerate}
\item
	\begin{enumerate}[label={\Alph*.}]
	\item \(\)
	\item \(\)
	\item \(\)
	\item \(\)
	\end{enumerate}
\item
	\begin{enumerate}[label={\Alph*.}]
	\item \(\)
	\item \(\)
	\item \(\)
	\item \(\)
	\end{enumerate}
\item
	\begin{enumerate}[label={\Alph*.}]
	\item \(\)
	\item \(\)
	\item \(\)
	\item \(\)
	\end{enumerate}
\item
	\begin{enumerate}[label={\Alph*.}]
	\item \(\)
	\item \(\)
	\item \(\)
	\item \(\)
	\end{enumerate}
\item
	\begin{enumerate}[label={\Alph*.}]
	\item \(\)
	\item \(\)
	\item \(\)
	\item \(\)
	\end{enumerate}
\item
	\begin{enumerate}[label={\Alph*.}]
	\item \(\)
	\item \(\)
	\item \(\)
	\item \(\)
	\end{enumerate}
\item
	\begin{enumerate}[label={\Alph*.}]
	\item \(\)
	\item \(\)
	\item \(\)
	\item \(\)
	\end{enumerate}
\item
	\begin{enumerate}[label={\Alph*.}]
	\item \(\)
	\item \(\)
	\item \(\)
	\item \(\)
	\end{enumerate}
\item
	\begin{enumerate}[label={\Alph*.}]
	\item \(\)
	\item \(\)
	\item \(\)
	\item \(\)
	\end{enumerate}
\item
	\begin{enumerate}[label={\Alph*.}]
	\item \(\)
	\item \(\)
	\item \(\)
	\item \(\)
	\end{enumerate}
\end{enumerate}
\end{multicols}