\chapter{Calculus}
\section{Differentiation}
\subsection{Questions}
\begin{multicols}{2}
\begin{enumerate}[label={\arabic*.}]
  \item The minimum point on the curve \(y = x^2 - 6x + 5\) is at?
        \begin{enumerate}[label={\Alph*.}]
            \item (1,5)
            \item (2,3)
            \item (3,4)
            \item (-3,4)
            \item (3,-4)
        \end{enumerate}
  \item At what value of \(x\) is the function \(y = x^2 + x + 1\) minimum? 
        \begin{enumerate}[label={\Alph*.}]
            \item \(-1\)
            \item \(-\frac{1}{2}\)
            \item \(\frac{1}{2}\)
            \item \(1\)
        \end{enumerate}
  \item At what value of \(x\) is the function \(y = x^2 - 2x - 3\) minimum?
    \begin{enumerate}[label={\Alph*.}]
            \item \(1\) 
            \item  \(-1\) 
            \item \(-4\)
            \item \(4\)
        \end{enumerate}
  \item Find the maximum value of \(y = x^2 - 2x - 3\)
        \begin{enumerate}[label={\Alph*.}]
			\item \(-4\)
			\item \(-1\)
			\item \(1\)
			\item \(4\)
        \end{enumerate}
  \item Find the maximum value of \(y = 3x^2 - x^3\)
        \begin{enumerate}[label={\Alph*.}]
            \item \(2\)
            \item \(4\)
            \item \(6\)
            \item \(0\)
        \end{enumerate}
  \item Find the minimum value of \(y = x^3 + x^2 - x + 1\)
        \begin{enumerate}[label={\Alph*.}]
            \item \(\)
			\item \(\)
			\item \(\)
			\item \(\)
			\item \(\)
        \end{enumerate}
  \item Find the value of \(x\) for which the function \(f(x) = 2x^3 - x^2 -4x + 4\) has a maximum value.
        \begin{enumerate}[label={\Alph*.}]
            \item \(\frac{2}{3}\)
            \item \(1\)
            \item \(-1\)
            \item \(-\frac{2}{3}\)
        \end{enumerate}
  \item Find the value of \(x\) for which the function \(f(x) = 3x^3-9x^2\) is minimum
        \begin{enumerate}[label={\Alph*.}]
            \item \(2\)
            \item \(0\)
            \item \(5\)
            \item \(3\)
        \end{enumerate}
  \item Find the maximum value of the function \(f(x) = 2 + x - x^2\)
        \begin{enumerate}[label={\Alph*.}]
            \item \(\frac{9}{4}\)
            \item \(\frac{7}{4}\)
            \item \(\frac{3}{2}\)
            \item \(\frac{1}{2}\)
        \end{enumerate}
  \item Find the maximum value of \(y\) in the equation: \(y = 1 - 2 - 3x^2\)
        \begin{enumerate}[label={\Alph*.}]
            \item \(\frac{4}{3}\)
            \item \(\frac{5}{4}\)
            \item \(\frac{3}{4}\)
            \item \(\frac{5}{3}\)
        \end{enumerate}
  \item The minimum value of \(y\) in the equation: \(y = x^2 - 6x + 8\) is
        \begin{enumerate}[label={\Alph*.}]
            \item \(8\)
            \item \(3\)
            \item \(0\)
            \item \(-1\)
        \end{enumerate}
  \item Obtain a maximum value of the function: \(f(x) = x^3 - 12x + 11\)
        \begin{enumerate}[label={\Alph*.}]
            \item \(-5\)
            \item \(-2\)
            \item \(2\)
            \item \(27\)
        \end{enumerate}
  \item Find the value of \(h\) if the maximum value of \(y = 1 + hx - 3x^2\) is 13.
        \begin{enumerate}[label={\Alph*.}]
            \item \(10\)
            \item \(11\)
            \item \(12\)
            \item \(13\)
        \end{enumerate}
  \item A trader realizes \(10x - x^2\) naira profit from the sale of \(x\) bags of corn. How many bags will give him the maximum profit?
        \begin{enumerate}[label={\Alph*.}]
            \item \(4\)
            \item \(5\)
            \item \(6\)
            \item \(7\)
        \end{enumerate}
  \item Find the value of \(x\) for which the function \(y = x^3 - x\) has a minimum value.
        \begin{enumerate}[label={\Alph*.}]
            \item \(\frac{\sqrt{3}}{3}\)
            \item -\(\frac{\sqrt{3}}{3}\)
            \item \(\sqrt{3}\)
            \item -\(\sqrt{3}\)
        \end{enumerate}
  \item If \(f(x) = x^2 - 2x - 3\), find the least value of \(f(x)\) and the corresponding value of \(x\).
        \begin{enumerate}[label={\Alph*.}]
            \item \(f(x) = -3, x = 1\)
            \item \(f(x) = -3, x = 3\)
            \item \(f(x) = 1, x = -4\)
            \item \(f(x) = 1, x = -4\)
        \end{enumerate}
  \item If \(y = 3 \cos\left(\frac{x}{3}\right)\), find \(\dv{y}{x}\) when \(x = \frac{3\pi}{2}\).
        \begin{enumerate}[label={\Alph*.}]
            \item \(-1\)
            \item \(1\)
            \item \(2\)
            \item  \(3\)
        \end{enumerate}
  \item What is the rate of change of the volume \(v\) of a hemisphere with respect to its radius \(r\) when \(r = 2\)?
        \begin{enumerate}[label={\Alph*.}]
            \item  \(2\pi\)
            \item  \(4\pi\)
            \item  \(8\pi\)
            \item  \(16\pi\)
        \end{enumerate}
  \item If \(y = (1-2x)^3\), find the value of \(\dv{y}{x}\) at \(x = -1\).
         \begin{enumerate}[label={\Alph*.}]
            \item  \(22\)
            \item \(57\)
            \item \(-6\)
            \item \(-54\)
        \end{enumerate}
  \item Find the derivative of \(y = \sin(2x^3+3x-4)\).
      \begin{enumerate}[label={\Alph*.}]
            \item \(\cos(2x^2+3x-4)\)
            \item \(-\cos(2x^2+3x-4)\)
            \item  \(-(6x^2+3)\cos(2x^2+3x-4)\)
            \item \((6x^2 + 3) \cos(2x^2+3x-4)\)
        \end{enumerate}
  \item The radius \(r\) of a circular disc is increasing at the rate of \(0.5\ \text{cm/sec}\). At what rate is the area of the disc increasing when its radius is \(6\ \text{cm}\)?
       \begin{enumerate}[label={\Alph*.}]
            \item  \(3\pi\ \text{cm}^2/\text{sec}\)
            \item  \(18\pi\ \text{cm}^2/\text{sec}\)
            \item  \(6\pi\ \text{cm}^2/\text{sec}\)
            \item \(36\pi\ \text{cm}^2/\text{sec}\)
        \end{enumerate}
  \item Find \(\dv{y}{x}\), if \(y = \cos x\).
       \begin{enumerate}[label={\Alph*.}]
            \item  \(\sin x\)
            \item  \(-\sin x\)
            \item  \(\tan x\)
            \item  \(-\tan x\)
        \end{enumerate}
  \item Differentiate: \((\cos \theta - \sin \theta)^2\) with respect to \(\theta\).
     \begin{enumerate}[label={\Alph*.}]
            \item \(1-2\cos 2\theta\)
            \item  \(-2\sin 2\theta\)
            \item  \(-2\cos 2\theta\)
            \item  \(1-2\sin 2\theta\)
        \end{enumerate}
  \item Differentiate: \(\left(x^2 + \frac{1}{x}\right)^2\) with respect to \(x\).
       \begin{enumerate}[label={\Alph*.}]
            \item \(4x^3 - 2 + \frac{2}{x^3}\)
            \item  \(4x^3 - 2 - \frac{2}{x^3}\)
            \item   \(4x^3 - 4x - \frac{2}{x}\)
            \item    \(4x^3 - 3x + \frac{2}{x}\)
        \end{enumerate}
\item Find the point \(x,y\) on the Euclidean plane where the curve \(y = 2x^{2} - 2x +3\) has \(2\) as the gradient.
    \begin{enumerate}[label={\Alph*.}]
        \item \((1, 4)\)
        \item \((2, 2)\)
        \item \((3, 4)\)
        \item \((3, 2)\)
    \end{enumerate}  
\item For what value of \(x\) is the tangent to the curve \(y = x^{2} - 4x + 3\) parallel to the \(x\)-axis?
    \begin{enumerate}[label={\Alph*.}]
        \item \(0\)
        \item \(1\)
        \item \(2\)
        \item \(3\)
    \end{enumerate}   
\item If \(y = x \sin x\), find \( \frac{d^2y}{dx^2} \).
	\begin{enumerate}[label={\Alph*.}]
	\item \(2\cos x - \sin x\)
	\item \(\sin x + \cos x\)
	\item \(\sin x  - \cos  x\)
	\item \( \cos x  - 2\sin x \)
	\end{enumerate}
\item Differentiate: \(\frac{6x^{3} - 5x^{2} + 1}{3x^{2}}\) with respect to \(x\)
	\begin{enumerate}[label={\Alph*.}]
	\item \(2 + \frac{2}{3{x}^{3}}\)
	\item \(2 + \frac{1}{6x}\)
	\item \(\sin x - \cos x\)
	\item \(\cos x - 2\sin x\)
	\end{enumerate}
\item If \(y = (1+x)^{2}\), find \( \dv{y}{x} \).
	\begin{enumerate}[label={\Alph*.}]
	\item \(x+1\)
	\item \(2x-1\)
	\item \(2 + 2x\)
	\item \(1+2x\)
	\end{enumerate}
\item Differentiate: \(3x^3+2x^2+3x+1\) with respect to \(x\)
	\begin{enumerate}[label={\Alph*.}]
	\item \(9x^2+4x+3\)
	\item \(9x^2+4x-3\)
	\item \(9x^2-4x-3\)
	\item \(9x^2-4x+3\)
	\end{enumerate}
\item Differentiate: \(\frac{2}{3}x^{3}-\frac{4}{x}\)
	\begin{enumerate}[label={\Alph*.}]
	\item \(2x^2 + \frac{4}{x^2}\)
	\item \(2x^{2}-\frac{4}{x}\)
	\item \(3x^{2}-\frac{4}{x}\)
	\item \(3x^{2}+\frac{4}{x^2}\)
	\end{enumerate}
\item Find the derivative of \(\frac{\sin {x}}{\cos {x}}\)
	\begin{enumerate}[label={\Alph*.}]
	\item \(\tan{x}\cos{x}\)
	\item \(\csc{x}\sec{x}\)
	\item \(\sec^{2}{x}\)
	\item \(\cot^{2}{x}\)
	\end{enumerate}
\item If \(y=x^2-3x+4\), find \(\dv{y}{x}\) at \(x=5\).
	\begin{enumerate}[label={\Alph*.}]
	\item \(9\)
	\item \(7\)
	\item \(5\)
	\item \(3\)
	\end{enumerate}
\item If \(y= 2x\cos{2x} -\sin{2x}\), find \(\dv{y}{x}\) when \(x=\frac{\pi}{4}\).
	\begin{enumerate}[label={\Alph*.}]
	\item \(9\)
	\item \(7\)
	\item \(5\)
	\item \(3\)
	\end{enumerate}
\item If \(y=3\cos{4x}\), find \(\dv{y}{x}\)
	\begin{enumerate}[label={\Alph*.}]
	\item \(-24\sin{4x}\)
	\item \(12\sin{4x}\)
	\item \(-12 \sin{4x}\)
	\item \(6\sin{8x}\)
	\end{enumerate}
\item Find the derivative of \((2+3x)(1-x)\) with respect to \(x\).
	\begin{enumerate}[label={\Alph*.}]
	\item \(6x-1\)
	\item \(1-6x\)
	\item \(-3\)
	\item \(6\)
	\end{enumerate}
\item Find \(\dv{y}{x}\), if \(y = 3{x}^{3}+2{x}^{2}+3x+1\).
	\begin{enumerate}[label={\Alph*.}]
	\item \(9{x}^{2}+4{x}+3\)
	\item \(9{x}^{2}+4{x}-3\)
	\item \(9{x}^{2}-4{x}+3\)
	\item \(9{x}^{2}-4{x}-3\)
	\end{enumerate}
\item If \(y = 2{x}^{3}+6{x}^{2}+6x+1\), find \(\dv{y}{x}\).
	\begin{enumerate}[label={\Alph*.}]
	\item \(6{x}^{2}+12{x}+1\)
	\item \(6{x}^{2}-12{x}+1\)
	\item \(6{x}^{2}+12{x}+6\)
	\item \(6{x}^{2}+6{x}+6\)
	\end{enumerate}
\item Find the derivative of \(y ={\left(\dfrac{1}{3}x + 6\right)}^{2}\).
	\begin{enumerate}[label={\Alph*.}]
	\item \(2{\left(\dfrac{1}{3}x + 6\right)}\)
	\item \(\frac{2}{3}{\left(\dfrac{1}{3}x + 6\right)}\)
	\item \(\frac{1}{3}{\left(\dfrac{1}{3}x + 6\right)}^{2}\)
	\item \(\frac{2}{3}{\left(\dfrac{1}{3}x + 6\right)}^{2}\)
	\end{enumerate}
\item If \(y = {x}^{2}-3{x}+4\), find \(\dv{y}{x}\) at \(x = 5\).
	\begin{enumerate}[label={\Alph*.}]
	\item \(9\)
	\item \(7\)
	\item \(5\)
	\item \(3\)
	\end{enumerate}
\item If  \(y = {x}^{2}+\sqrt{x}\), find \(\dv{y}{x}\).
	\begin{enumerate}[label={\Alph*.}]
	\item \(2x-\frac{1}{2}x^{\frac{1}{2}}\)
	\item \(2x-\frac{1}{2}x^{-{\frac{1}{2}}}\)
	\item \(2x+x^{-{\frac{1}{2}}}\)
	\item \(2x+\frac{1}{2}x^{-{\frac{1}{2}}}\)
	\end{enumerate}
\item Find \(\dv{y}{x}\), if \(y = \frac{2}{3}{x}^{3}-\frac{4}{x}\)
	\begin{enumerate}[label={\Alph*.}]
	\item \({3}{x}^{2}-\frac{4}{x}\)
	\item \({3}{x}^{2}+\frac{4}{x^{2}}\)
	\item \({2}{x}^{2}-\frac{4}{x}\)
	\item \({2}{x}^{2}+\frac{4}{x^{2}}\)
	\end{enumerate}
\item If \(y = \cos{(3x)}\), find \(\dv{y}{x}\).
	\begin{enumerate}[label={\Alph*.}]
	\item \(\frac{1}{3}\sin{(3x)}\)
	\item \({3}\sin{(3x)}\)
	\item \(-{\frac{1}{3}}\sin{(3x)}\)
	\item \(-3\sin{(3x)}\)
	\end{enumerate}
\item Find \(\dv{y}{x}\), if \(y = \cos{x}\)
	\begin{enumerate}[label={\Alph*.}]
	\item \(\sin{x}\)
	\item \(-\sin{x}\)
	\item \(\tan{x}\)
	\item \(-\tan{x}\)
	\end{enumerate}
\item Find the slope of the curve: \(y = 2x^{3}+ 5{x}-3\) at \((1,4)\).
	\begin{enumerate}[label={\Alph*.}]
	\item \(4\)
	\item \(6\)
	\item \(7\)
	\item \(9\)
	\end{enumerate}
\item Find the derivative of \(y = \sin^{2}{(5x)}\) with respect to \(x\).
	\begin{enumerate}[label={\Alph*.}]
	\item \(5 \sin{(5x)\cos{(5x)}}\)
	\item \(2 \sin{(5x)\cos{(5x)}}\)
	\item \(15 \sin{(5x)\cos{(5x)}}\)
	\item \(10 \sin{(5x)\cos{(5x)}}\)
	\end{enumerate}
\item The slope of the tangent to the curve: \(y=3{x}^{2}-2x+5\) at the point \((1,6)\) is
	\begin{enumerate}[label={\Alph*.}]
	\item \(1\)
	\item \(4\)
	\item \(5\)
	\item \(6\)
	\end{enumerate}
\item If the gradient of the curve \(y=2k{x}^{2}+x+1\) at \(x = 1\) is 9, find the value of \(k\)
	\begin{enumerate}[label={\Alph*.}]
	\item \(\)
	\item \(\)
	\item \(\)
	\item \(\)
	\end{enumerate}
\item Find the 
	\begin{enumerate}[label={\Alph*.}]
	\item \(\)
	\item \(\)
	\item \(\)
	\item \(\)
	\end{enumerate}
\item
	\begin{enumerate}[label={\Alph*.}]
	\item \(\)
	\item \(\)
	\item \(\)
	\item \(\)
	\end{enumerate}
\item
	\begin{enumerate}[label={\Alph*.}]
	\item \(\)
	\item \(\)
	\item \(\)
	\item \(\)
	\end{enumerate}
\item
	\begin{enumerate}[label={\Alph*.}]
	\item \(\)
	\item \(\)
	\item \(\)
	\item \(\)
	\end{enumerate}
\item
	\begin{enumerate}[label={\Alph*.}]
	\item \(\)
	\item \(\)
	\item \(\)
	\item \(\)
	\end{enumerate}
\item
	\begin{enumerate}[label={\Alph*.}]
	\item \(\)
	\item \(\)
	\item \(\)
	\item \(\)
	\end{enumerate}
\item
	\begin{enumerate}[label={\Alph*.}]
	\item \(\)
	\item \(\)
	\item \(\)
	\item \(\)
	\end{enumerate}
\item
	\begin{enumerate}[label={\Alph*.}]
	\item \(\)
	\item \(\)
	\item \(\)
	\item \(\)
	\end{enumerate}
\item
	\begin{enumerate}[label={\Alph*.}]
	\item \(\)
	\item \(\)
	\item \(\)
	\item \(\)
	\end{enumerate}
\item
	\begin{enumerate}[label={\Alph*.}]
	\item \(\)
	\item \(\)
	\item \(\)
	\item \(\)
	\end{enumerate}
\item
	\begin{enumerate}[label={\Alph*.}]
	\item \(\)
	\item \(\)
	\item \(\)
	\item \(\)
	\end{enumerate}
\item
	\begin{enumerate}[label={\Alph*.}]
	\item \(\)
	\item \(\)
	\item \(\)
	\item \(\)
	\end{enumerate}
\item
	\begin{enumerate}[label={\Alph*.}]
	\item \(\)
	\item \(\)
	\item \(\)
	\item \(\)
	\end{enumerate}
\item
	\begin{enumerate}[label={\Alph*.}]
	\item \(\)
	\item \(\)
	\item \(\)
	\item \(\)
	\end{enumerate}
\item
	\begin{enumerate}[label={\Alph*.}]
	\item \(\)
	\item \(\)
	\item \(\)
	\item \(\)
	\end{enumerate}
\item
	\begin{enumerate}[label={\Alph*.}]
	\item \(\)
	\item \(\)
	\item \(\)
	\item \(\)
	\end{enumerate}
\item
	\begin{enumerate}[label={\Alph*.}]
	\item \(\)
	\item \(\)
	\item \(\)
	\item \(\)
	\end{enumerate}
\item
	\begin{enumerate}[label={\Alph*.}]
	\item \(\)
	\item \(\)
	\item \(\)
	\item \(\)
	\end{enumerate}
\item
	\begin{enumerate}[label={\Alph*.}]
	\item \(\)
	\item \(\)
	\item \(\)
	\item \(\)
	\end{enumerate}
\item
	\begin{enumerate}[label={\Alph*.}]
	\item \(\)
	\item \(\)
	\item \(\)
	\item \(\)
	\end{enumerate}
\item
	\begin{enumerate}[label={\Alph*.}]
	\item \(\)
	\item \(\)
	\item \(\)
	\item \(\)
	\end{enumerate}
\item
	\begin{enumerate}[label={\Alph*.}]
	\item \(\)
	\item \(\)
	\item \(\)
	\item \(\)
	\end{enumerate}
\item
	\begin{enumerate}[label={\Alph*.}]
	\item \(\)
	\item \(\)
	\item \(\)
	\item \(\)
	\end{enumerate}
\item
	\begin{enumerate}[label={\Alph*.}]
	\item \(\)
	\item \(\)
	\item \(\)
	\item \(\)
	\end{enumerate}
\item
	\begin{enumerate}[label={\Alph*.}]
	\item \(\)
	\item \(\)
	\item \(\)
	\item \(\)
	\end{enumerate}
\item
	\begin{enumerate}[label={\Alph*.}]
	\item \(\)
	\item \(\)
	\item \(\)
	\item \(\)
	\end{enumerate}
\item
	\begin{enumerate}[label={\Alph*.}]
	\item \(\)
	\item \(\)
	\item \(\)
	\item \(\)
	\end{enumerate}
\item
	\begin{enumerate}[label={\Alph*.}]
	\item \(\)
	\item \(\)
	\item \(\)
	\item \(\)
	\end{enumerate}
\item
	\begin{enumerate}[label={\Alph*.}]
	\item \(\)
	\item \(\)
	\item \(\)
	\item \(\)
	\end{enumerate}
\item
	\begin{enumerate}[label={\Alph*.}]
	\item \(\)
	\item \(\)
	\item \(\)
	\item \(\)
	\end{enumerate}
\item
	\begin{enumerate}[label={\Alph*.}]
	\item \(\)
	\item \(\)
	\item \(\)
	\item \(\)
	\end{enumerate}
\item
	\begin{enumerate}[label={\Alph*.}]
	\item \(\)
	\item \(\)
	\item \(\)
	\item \(\)
	\end{enumerate}
\item
	\begin{enumerate}[label={\Alph*.}]
	\item \(\)
	\item \(\)
	\item \(\)
	\item \(\)
	\end{enumerate}
\item
	\begin{enumerate}[label={\Alph*.}]
	\item \(\)
	\item \(\)
	\item \(\)
	\item \(\)
	\end{enumerate}
\item
	\begin{enumerate}[label={\Alph*.}]
	\item \(\)
	\item \(\)
	\item \(\)
	\item \(\)
	\end{enumerate}
\item
	\begin{enumerate}[label={\Alph*.}]
	\item \(\)
	\item \(\)
	\item \(\)
	\item \(\)
	\end{enumerate}
\item
	\begin{enumerate}[label={\Alph*.}]
	\item \(\)
	\item \(\)
	\item \(\)
	\item \(\)
	\end{enumerate}
\item
	\begin{enumerate}[label={\Alph*.}]
	\item \(\)
	\item \(\)
	\item \(\)
	\item \(\)
	\end{enumerate}
\item
	\begin{enumerate}[label={\Alph*.}]
	\item \(\)
	\item \(\)
	\item \(\)
	\item \(\)
	\end{enumerate}
\item
	\begin{enumerate}[label={\Alph*.}]
	\item \(\)
	\item \(\)
	\item \(\)
	\item \(\)
	\end{enumerate}
\item
	\begin{enumerate}[label={\Alph*.}]
	\item \(\)
	\item \(\)
	\item \(\)
	\item \(\)
	\end{enumerate}
\item
	\begin{enumerate}[label={\Alph*.}]
	\item \(\)
	\item \(\)
	\item \(\)
	\item \(\)
	\end{enumerate}
\item
	\begin{enumerate}[label={\Alph*.}]
	\item \(\)
	\item \(\)
	\item \(\)
	\item \(\)
	\end{enumerate}
\item
	\begin{enumerate}[label={\Alph*.}]
	\item \(\)
	\item \(\)
	\item \(\)
	\item \(\)
	\end{enumerate}
\item
	\begin{enumerate}[label={\Alph*.}]
	\item \(\)
	\item \(\)
	\item \(\)
	\item \(\)
	\end{enumerate}
\item
	\begin{enumerate}[label={\Alph*.}]
	\item \(\)
	\item \(\)
	\item \(\)
	\item \(\)
	\end{enumerate}
\item
	\begin{enumerate}[label={\Alph*.}]
	\item \(\)
	\item \(\)
	\item \(\)
	\item \(\)
	\end{enumerate}
\item
	\begin{enumerate}[label={\Alph*.}]
	\item \(\)
	\item \(\)
	\item \(\)
	\item \(\)
	\end{enumerate}
\item
	\begin{enumerate}[label={\Alph*.}]
	\item \(\)
	\item \(\)
	\item \(\)
	\item \(\)
	\end{enumerate}
\item
	\begin{enumerate}[label={\Alph*.}]
	\item \(\)
	\item \(\)
	\item \(\)
	\item \(\)
	\end{enumerate}
\item
	\begin{enumerate}[label={\Alph*.}]
	\item \(\)
	\item \(\)
	\item \(\)
	\item \(\)
	\end{enumerate}
\item
	\begin{enumerate}[label={\Alph*.}]
	\item \(\)
	\item \(\)
	\item \(\)
	\item \(\)
	\end{enumerate}
\end{enumerate}
\end{multicols}