\subsection{Solution}
\begin{multicols}{2}
\begin{enumerate}[label={\textbf{\arabic*.}}]
    \item We begin by converting all the mixed fractions to improper fractions and add them up.\\
    \[3\dfrac{7}{8} = \dfrac{31}{8} \text { and } 1\dfrac{1}{3} = \dfrac{4}{3}\] \\ 
    Taking LCM of \(8\) and \(3\) we get \(24\),
    \begin{align*}
    \frac{31}{8} + \frac{4}{3} &= \frac{(31 \times 3) + (8 \times 4) }{24} \\
    &= \frac{93 + 32}{24} = \dfrac{125}{24}
    \end{align*}
    Similarly, 
    \[1\frac{2}{3} - \frac{3}{8} \Rightarrow \frac{5}{3} - \frac{3}{8} = \frac{(5 \times 8) - (3 \times 3)}{24} = \frac{31}{24}\]
    Now subtract \(\dfrac{31}{24} \text { from } \dfrac{125}{24}\)
    \[\frac{125}{24} - \frac{31}{24} = \frac{125 - 31}{24} = \frac{94}{24} = 3\frac{11}{12} \text{(D)} \]
    
    \item \textbf{Amount he earned before the increase} i.e his Initial Salary \\
    Let initial Salary = \(x\) \hspace {10px}  new salary = N345\\
    So, listen He had 15\% of his initial salary (x) added to his initial earn (x)
    \[\text{initial salary + 15\% of initial = new salary}\]
    \begin{align*}
    x + \dfrac{15}{100}x = 345 &\Rightarrow \dfrac{100x + 15x}{100} = 345 \\
    115x = 345 \times 100 &\Rightarrow x = \left(\frac{345}{115}\right) \times 100 \\
    \therefore \hspace{70px} 3 \times 100 &= 300 \text{ (B)}\\
    \end{align*}
    \textbf{Note:} when give this: \( \dfrac{x \times 100}{y}\)its advisable to group in the form
    \(\left(\dfrac{x}{y}\right) \times 100\) , incase the fraction part becomes decimal the 100 only shift the
    decimal point. 

    \item \textbf{(C) } $ \sqrt{41830}$ is not a perfect square, so we can't evaulate using tables
    \[ \sqrt{41830} \approx 204.5 = 205 \hspace{30px} \text{\{ to 3d.p\}}\]
    \item The \textbf{time taken (t)} to complete a job is inversely proportional to \textbf{numbers ot men (n)} 
    i.e as the number of men increase the job is done faster. 
    \begin{equation}
        \text{time taken} \propto \dfrac{1}{\text{number of men}} \Rightarrow t \propto \dfrac{1}{n}
    \end {equation}
    Removing proportionality sign
    \[t = \dfrac{k}{n} \Rightarrow tn = k\]
    Generally: \(t_{1}n_{1} = t_{2}n_2 = \cdots = t_{k}n_{k}\)\\
    given \(t_{1} = 9\ , n_{1} = 12 , t_{2} = 6 \text{ and } n_{2} = ?\) \\
    Using: \(t_{1}n_{1} = t_{2}n_{2} \Rightarrow 9 \times 12 = 6 \times n_{2}\) \\
    taking the advantage that 6 $\mid$ 12 
    \[n_{2} = \left(\frac{12}{6}\right) \times 9 = 18 \text { men (E)}\]

    \item Remember convert to improper fraction first
    \[2\frac{5}{12} - 1\frac{7}{8} \times \frac{6}{5} \Rightarrow \frac{29}{12} - \frac{15}{8} \times \frac{6}{5}\]
    Applying BODMAS multilplication comes before substraction\\
    \[\therefore  \dfrac{29}{12} - \left(\dfrac{\cancelto{3}{15} \times \cancelto{3}{6}}{\cancelto{4}{8} \times \cancelto{1}{5}}\right) \Rightarrow \dfrac{29}{12} - \dfrac{9}{4} = \dfrac{29 - (9 \times 3)}{12} = \frac{2}{12} = \frac{1}{6} \text{(C)}\]

    \item \textbf{(B)} Selling Price = N45.00, profit\% = 8\%, let cost price = \(x\)
    \begin{align*}
    \%\text{profit} &= \frac{\text{Selling Price - Cost Price} }{\text{Cost Price}} \times 100 \\
       \Rightarrow \hspace*{60px}  8 &= \frac{45 - x }{x} \times 100 \\
        8x &= 4500 -100x\\
       108x &= 4500 \\ 
       x &= \dfrac{4500}{108}  \\
       \therefore \hspace{25px}  \text{ cost price }  &= \dfrac{4500}{108} \\
    \end{align*}
       Now the question says He had made a \%profit of 32\%, how much did he sell it? \\
       Using Formular, We have: \\
       \begin{align*}
        32 &= \dfrac{SP - \dfrac{4500}{108}}{\dfrac{4500}{108}} \times 100 \\
        &= \dfrac{108\left(SP - \dfrac{4500}{108}\right)}{4500} \times 100 \\
        &=  \dfrac{108SP - 4500}{4500} \times 100 \\
        \dfrac{32 \times 4500}{100} &= 108SP - 4500 \\
        SP &= \dfrac{\left(32 \times 45\right) + 4500}{108} \\ 
        &= \dfrac{5940}{108} = 55 
        \end{align*}
    \item \textbf{(B) }The easiest ways is to compare $\dfrac{1}{3}$ with every other item \\
        \begin{align*}
            \dfrac{4}{11} \text{ vs } \dfrac{1}{3} &\Rightarrow \dfrac{4}{11} \text{ vs } \dfrac{4}{12} \\
            \dfrac{122}{383} \text{ vs } \dfrac{1}{3} &\Rightarrow \dfrac{122}{383} \text{ vs } \dfrac{122}{366} \\
            \dfrac{15}{44} \text{ vs } \dfrac{1}{3} &\Rightarrow \dfrac{15}{44} \text{ vs } \dfrac{15}{45} \\
            \dfrac{22}{63} \text{ vs } \dfrac{1}{3} &\Rightarrow \dfrac{22}{63} \text{ vs } \dfrac{22}{66} \\
            \dfrac{6}{14} \text{ vs } \dfrac{1}{3} &\Rightarrow \dfrac{6}{14} \text{ vs } \dfrac{6}{18} \\
        \end{align*}
        Since the denominator in $\dfrac{122}{383}$ is greater than $\dfrac{122}{366} = \dfrac{1}{3}$ therefore $\dfrac{122}{383}$ is lessthan one-third

    \item \textbf{In 1980:} The intial price \(a : x\) rose by 25\% and 10\% respectively, hence:
    \[a:x \Rightarrow  a + \dfrac{25}{100}a : x + \dfrac{10}{100}x\]
    Which reduces to \(\dfrac{125}{\cancel{100}}a : \dfrac{110}{\cancel{100}}x \Rightarrow {125}a : 110x  \) \vspace{5px} \\
    dividing by 5 \(\dfrac{\cancelto{25}{125}}{\cancel{5}} a : \dfrac{\cancelto{22}{110}}{\cancel{5}} x \hspace {10px}\Rightarrow 25a : 22x \) \vspace{5px}\\
    Multiplying by 2  \(50a : 44x\) \hspace{5px}Option (A)
    \[\]

    \item For Questions like this its best to start from the bottom \\
    \textbf{Pre-requesite:} \\
    \begin{align*}
    &5 + \dfrac{6}{7} =  \dfrac{41}{7} \\
    &4 \divisionsymbol \dfrac{41}{7} = \dfrac{28}{41} \\
    &3 + \dfrac{28}{41} = \dfrac{151}{41} \\
    &2 \divisionsymbol \dfrac{151}{41} = \dfrac{82}{151}\\
    &1 + \dfrac{82}{151} = \dfrac{233}{151} \\ 
    \end{align*}
    
    \item \textbf{(C)}\begin{align*}
        827.51 \times 15 \times 10^{-3} &= 12.41265 \\
        &= 12.4127 \hspace{30px} \text{\{ to 4d.p\}}
        \end{align*}
    \item Notice the difference between million and million\textbf{th}
    \begin{align*}
    \text{  i.e } \hspace{40px} 1 \text{micrometer} &= 10^{-6}\text{millimeter} \\
    12,000 \text{micrometer} &= x \text{ millimeter} \\
    x &= 12000 \times 10^{-6}  \\
    &= 1.2 \times 10^{-4 -6 } \\
    &= 1.2 \times 10^{-10} \\
    \text{i.e} \hspace{88px}  x &= 0.00000000012 \text{m}
    \end{align*}

    \item Converting to improper fraction 
    \begin{align*}
        4\dfrac{5}{7} - 2\dfrac{1}{4} &\Rightarrow \dfrac{33}{7} - \dfrac{9}{4} \\
        \text{Taking LCM:} \hspace{20px}\\
        \dfrac{(33\times 4) - (9 \times 7) }{28} &= \dfrac{132 - 63}{28} = \dfrac{69}{28} \\
        \dfrac{1}{14} + 1\dfrac{1}{2} &= \dfrac{1}{14} + \dfrac{3}{2} \\
        &= \dfrac{1 + (7 \times 3)}{14} = \dfrac{22}{14} \\
        \Rightarrow \hspace{30px} \dfrac{69}{28} - \dfrac{22}{14} &= \dfrac{69 - (22 \times 2)}{28} =  \dfrac{25}{28} = \dfrac{50}{56} \text{ (C) }
    \end{align*}

    \item SP = N81, \%profit = 8\% \\
    What did he pay for the bicycle = \textbf{CP} = x \\
    \begin{align*}
    \%\text{profit} &= \dfrac{ \text{SP - CP}}{\text{CP}} \times 100  \\ 
    \Rightarrow \hspace{55px} 8 &= \dfrac{81 - x }{x} \times 100 \\
     \hspace{50px} 8x &= 100(81 - x)  \\
     \hspace{50px} 2x &= 25(81 - x ) = (81\times25) -25x \\
     \hspace{50px} 27x &= 81\times 25 \\
    \therefore \hspace{60px}  x &= \dfrac{81 \times 25}{27} = \text{N}75
    \end{align*}

    \item  let CP = 400, woman's money = 10\% of 400 = N40 \\
    the remainder is supposed to be N360, but the man has 40\% of 360 = \(\dfrac{4\cancel{0}}{1\cancel{0}\cancel{0}} \times 36\cancel{0} = 144 \) \vspace {5px}\\
    So, answer is 40 + 144 = 184

    \item \textbf{(A)} Note that the same amount was invested in both cases and that amount is the principal(P) 
    \( \therefore \text{P}_1 = \text{P}_2\)
    \begin{align*} 
        \Rightarrow \hspace{40px} A_1 = P_1 + I_1 &= P_1 + \dfrac{P_1 \times R_1 \times T_1}{100} \\
        285.20&= P_1 + \dfrac{P_1 \times 5 \times 3}{100} \\
         28520 &= 100P_1 + 15P_1 = 115P_1 \\
         \dfrac{28520}{115}&= P_1 = 248 \\
        \Rightarrow \hspace{40px} A_2 = P_2 + I_2 &= P_2 + \dfrac{P_2 \times R_2 \times T_2}{100} \\
        434&= P_2 + \dfrac{P_2 \times 7\dfrac{1}{2} \times T_2}{100} \\
        \{ \because P_1 = P_2\} \hspace{40px} 434&= 248 + \dfrac{248 \times 7\dfrac{1}{2} \times T_2}{100} \\
        186 &= \dfrac{248 \times 15 \times T_2}{100 \times 2} \\
        \therefore \hspace{70px} T_2 & = 10 \text{ years}
    \end{align*}
    
    \item \textbf{(A) } Given that, \(B = A \text{ + 5000 and } \dfrac{A}{B} = \dfrac{4}{5}\), we are to find the sum 
    of the total profit $\left( A + B\right)$
    \[B = \dfrac{5}{9}(A + B) \text{ and } A = \dfrac{4}{9}(A + B)\]
    \begin{align*}
        B - A &= 5000 \\
        \dfrac{5}{9}(A + B) - \dfrac{4}{9}(A + B) &= 5000 \\
        \therefore \hspace{80px}  A + B &= 45000
    \end{align*}
    \item  
    \item \textbf{(B)} Start by resolving \\
    \[ \dfrac{4}{5} + \dfrac{1}{2} = \dfrac{13}{10}\text{now }  \dfrac{2}{13/10} = \dfrac{20}{13} \] 
    then, \\
    \[3 - \dfrac{20}{13} = \dfrac{39 - 20}{13} = \dfrac{19}{13} = 1\dfrac{6}{13} \]
    \item Given $\dfrac{x}{y} = \dfrac{1/3}{1/2} = \dfrac{2}{3} = \dfrac{28}{42}$ and $\dfrac{\psi}{\theta} = \dfrac{2/5}{4/7} = \dfrac{42}{60}$ \\
    \[ \hspace{10px} \dfrac{x/y}{\theta / \psi} = \left(\dfrac{x}{y}\right) \cdot \left(\dfrac{\psi}{\theta}\right) = \dfrac{28 \cdot \cancel{42}}{\cancel{42} \cdot 60} = \dfrac{7}{15}  \]
    \[\therefore \hspace{10px} x:\theta = 7:15\]
    \textbf{Note} I multiplied $y$ and $\psi$ by 14 and 3 respectively, so that they cancel each other
    \item 
    \item 
    \item 
    \item 
    \item
    \item
    \item
    \item 
    \item
    \item
    \item 
    \item 
    \item 
    \item 
    \item
    \item
    \item
    \item 
    \item
    \item
    \item 
    \item 
    \item 
    \item 
    \item
    \item
    \item
    \item 
    \item
    \item
    \item 
    \item 
    \item 
    \item 
    \item
    \item
    \item
    \item 
    \item
    \item
    \item 
    \item 
    \item 
    \item 
    \item
    \item
    \item
    \item 
    \item
    \item
    \item 
    \item 
    \item 
    \item 
    \item
    \item
    \item
    \item 
    \item
    \item
    \item 
    \item 
    \item 
    \item 
    \item
    \item
    \item
    \item 
    \item
    \item
    \item 
    \item 
    \item 
    \item 
    \item
    \item
    \item
    \item 
    \item
    \item
    \item 
    \item 
\end{enumerate}
\end {multicols}