\section{Indices and Standard Form}
\subsection{Questions}
\begin{multicols}{2}
\begin{enumerate}[label={\arabic*.}] 
\item If $(25)^{x-1} = 64\left(\cfrac{5}{2}\right)^6$, then $x$ has the value
	\begin{enumerate}[label={\Alph*.}]
	\item \(7\)
	\item \(4\)
	\item \(32\)
	\item \(5\)
	\item \(64\)
	\end{enumerate}
\item Simplify \(\cfrac{5^x \times 25^{x -1}}{125^{x+1}}\)
	\begin{enumerate}[label={\Alph*.}]
	\item \(5^{x+2}\)
	\item \(5^{2x -1}\)
	\item \(5^{x+1}\)
	\item \(5^3\)
	\item \(5^{-5}\)
	\end{enumerate}
\item Express $37.05 \times 0.0042$ in standard form 
	\begin{enumerate}[label={\Alph*.}]
	\item \(15.561 \times 10^2\)
	\item \(1.556 \times 10^1\)
	\item \(1.5561 \times 10^{-4}\)
	\item \(1.5561 \times 10^{-1}\)
	\item \(1.5561 \times 10^2\)
	\end{enumerate}
\item Simplify: $\sqrt[3]{(64r^{-6})^\frac{1}{2}}$
	\begin{enumerate}[label={\Alph*.}]
	\item \(\cfrac{1}{2r}\)
	\item \(\cfrac{2}{r}\)
	\item \(2\)
	\item \(\cfrac{1}{2}\)
	\end{enumerate}
\item What are the values of $y$ that satisfy this equation:
\[9^y -4(3^y) + 3 = 0\]
	\begin{enumerate}[label={\Alph*.}]
	\item \(-1 \text{ and } 0\)
	\item \(1 \text{ and } 3\)
	\item \(0 \text{ and } 1\)
	\item \(-1 \text{ and } 1\)
	\end{enumerate}
\item Simplify:  $\cfrac{9^{\frac{1}{3}} \times 27^{-\frac{1}{2}}}{3^{-\frac{1}{6}} \times 3^{-\frac{2}{3}}}$
	\begin{enumerate}[label={\Alph*.}]
	\item \(\cfrac{1}{3}\)
	\item \(\cfrac{1}{9}\)
	\item \(3\)
	\item \(1\)
	\item \(9\)
	\end{enumerate}
\item If \(\sqrt{3^x} = \sqrt[3]{9}\)
	\begin{enumerate}[label={\Alph*.}]
	\item \(\cfrac{3}{4}\)
	\item \(\cfrac{4}{3}\)
	\item \(\cfrac{1}{3}\)
	\item \(\cfrac{2}{3}\)
	\item \(\cfrac{1}{2}\)
	\end{enumerate}
\item Find the value of $\left(4^{\frac{1}{2}}\right)^6$
	\begin{enumerate}[label={\Alph*.}]
	\item \(6\)
	\item \(2\)
	\item \(1\)
	\item \(4\)
	\item \(8\)
	\end{enumerate}
\item Simplify: $\cfrac{3(2^{n-1}) - 4(2^{n-1})}{2^{n+1} - 2^n}$
	\begin{enumerate}[label={\Alph*.}]
	\item \(-2^{n-1}\)
	\item \(2^{n+1}\)
	\item \(-2^1\)
	\item \(-2^{-1}\)
	\end{enumerate}
\item Evaluate: $\cfrac{27^{\frac{1}{3}} - 8^{\frac{2}{3}}}{16^{\frac{2}{4}} \times 2}$ 
	\begin{enumerate}[label={\Alph*.}]
	\item \(-\cfrac{1}{8}\)
	\item \(\cfrac{21}{7}\)
	\item \(\cfrac{23}{5}\)
	\item \(-\cfrac{23}{5}\)
	\item \(-\cfrac{23}{6}\)
	\end{enumerate}
\item If \(\cfrac{4^{x+3}}{16^{2x -3}} = 1\), find $x$
	\begin{enumerate}[label={\Alph*.}]
	\item \(1\)
	\item \(-1\)
	\item \(-3\)
	\item \(3\)
	\item \(-3\)
	\end{enumerate}
\item Evaluate without using tables: $(0.008)^{-\frac{1}{3}} \times (0.16)^{-\frac{3}{2}}$
	\begin{enumerate}[label={\Alph*.}]
	\item \(\cfrac{8}{625}\)
	\item \(8\)
	\item \(\cfrac{625}{8}\)
	\item \(\cfrac{1}{8}\)
	\end{enumerate}
\item Simplify: $\cfrac{3^n - 3^{n-1}}{3^3 \times 3^n - 27 \times 3^{n-1}}$
	\begin{enumerate}[label={\Alph*.}]
	\item \(0\)
	\item \(\cfrac{1}{27}\)
	\item \(3^n - 3^{n-1}\)
	\item \(1\)
	\item \(\cfrac{2}{27}\)
	\end{enumerate}
\item Evaluate and leave your answer in standard form: 
\[\sqrt{\cfrac{0.0048 \times 0.81 \times 10^{-7}}{0.027 \times 0.04 \times 10^6}}\]
	\begin{enumerate}[label={\Alph*.}]
	\item \(6 \times 10^{-14}\)
	\item \(6 \times 10^{-7}\)
	\item \(6 \times 10^7\)
	\item \(6 \times 10^{14}\)
	\end{enumerate}
\item If $3^{2y} - 6(3^y) = 27$, find $y$
	\begin{enumerate}[label={\Alph*.}]
	\item \(3\)
	\item \(-1\)
	\item \(2\)
	\item \(-3\)
	\item \(1\)
	\end{enumerate}
\item If it is given that $5^{x+1} + 5^x = 150$, then the value of $x$ is equal to
	\begin{enumerate}[label={\Alph*.}]
	\item \(2\)
	\item \(3\)
	\item \(\cfrac{1}{2}\)
	\item \(1\)
	\item \(4\)
	\end{enumerate}
\item Given that $10^{2n + 1} = 0.0000001$, find $n$
	\begin{enumerate}[label={\Alph*.}]
	\item \(-7\)
	\item \(-6\)
	\item \(-\cfrac{3}{4}\)
	\item \(4\)
	\item \(-4\)
	\end{enumerate}
\item The result of dividing $\left(\cfrac{x^a}{x^b}\right)^{a-b} \text{ by } \left(\cfrac{x^{a+b}}{x^{a-b}}\right)^{\frac{a^2}{b}}$
	\begin{enumerate}[label={\Alph*.}]
	\item \(\)
	\item \(\)
	\item \(\)
	\item \(\)
	\end{enumerate}
\item If $\sqrt[3]{81} = 3^x$, find the value of $x$
	\begin{enumerate}[label={\Alph*.}]
	\item \(\cfrac{4}{3}\)
	\item \(-\cfrac{4}{3}\)
	\item \(\cfrac{3}{4}\)
	\item \(-\cfrac{3}{4}\)
	\end{enumerate}
\item Simplify: $\cfrac{x(x+1)^{-\frac{1}{2}} -(x+1)^{\frac{1}{2}}}{(x+1)^{\frac{1}{2}}} $
	\begin{enumerate}[label={\Alph*.}]
	\item \(\cfrac{1}{x+1}\)
	\item \(-\cfrac{1}{x+1}\)
	\item \(\cfrac{1}{x}\)
	\item \(-\cfrac{1}{\sqrt{x+1}}\)
	\end{enumerate}
\item Express in standard form \, $$\cfrac{0.8 \times 0.8 \times 0.8 - 0.5 \times 0.5 \times 0.5}{0.8 \times 0.8 + 0.8 \times 0.5 + 0.5 \times 0.5}$$
	\begin{enumerate}[label={\Alph*.}]
	\item \(8 \times 10^{-1}\)
	\item \(4 \times 10^{-1}\)
	\item \(3 \times 10^{-1}\)
	\item \(1.3 \times 10^{-1}\)
	\end{enumerate}
\item Express in standard form $$\cfrac{69842 \times 69842 - 30158 \times 30158}{69842 - 30158}$$
	\begin{enumerate}[label={\Alph*.}]
	\item \(3.0158 \times 10^{-4}\)
	\item \(10^{-4}\)
	\item \(6.9842 \times 10^{-5}\)
	\item \(10^{-5}\)
	\item \(10^5\)
	\end{enumerate}
\item The value of $\cfrac{9^2 \times 18^4}{3^{16}}$ is:
	\begin{enumerate}[label={\Alph*.}]
	\item \(\cfrac{2}{3}\)
	\item \(\cfrac{4}{9}\)
	\item \(\cfrac{32}{243}\)
	\item \(\cfrac{16}{81}\)
	\end{enumerate}
\item If $m$ and $n$ are whole numbers such that $m^n = 121$ then $(m-1)^{n+1} = ?$
	\begin{enumerate}[label={\Alph*.}]
	\item \(10\)
	\item \(10^2\)
	\item \(10^3\)
	\item \(10^4\)
	\end{enumerate}
\item Simplify: $\cfrac{a^\frac{1}{2} + a^{-\frac{1}{2}}}{1-a} + \cfrac{1- a^{\frac{1}{2}}}{1+ \sqrt{a}}$
	\begin{enumerate}[label={\Alph*.}]
	\item \(\cfrac{a}{a-1}\)
	\item \(\cfrac{a-1}{2}\)
	\item \(\cfrac{2}{a-1}\)
	\item \(\cfrac{2}{1-a}\)
	\end{enumerate}
\item Simplify: $\left(\cfrac{1}{64}\right)^0 + (64)^{-\frac{1}{2}} + (-32)^{\frac{4}{5}}$
	\begin{enumerate}[label={\Alph*.}]
	\item \(17\frac{1}{8}\)
	\item \(11\frac{7}{8}\)
	\item \(17\frac{3}{8}\)
	\item \(17\frac{7}{8}\)
	\end{enumerate}
\item If $\left(\cfrac{x}{y}\right)^{5a-3} = \left(\cfrac{y}{x}\right)^{17-3a}$, what is the value of $a$
	\begin{enumerate}[label={\Alph*.}]
	\item \(-7\)
	\item \(-5\)
	\item \(0\)
	\item \(3\)
	\end{enumerate}
\item Evaluate: $\cfrac{(0.064 - 0.008)(0.16 -0.04)}{(0.16+0.08+0.04)(0.4+0.2)^3}$
	\begin{enumerate}[label={\Alph*.}]
	\item \(\cfrac{1}{3}\)
	\item \(3\)
	\item \(\cfrac{3}{2}\)
	\item \(\cfrac{2}{3}\)
	\end{enumerate}
\item The value of $\left[\left(\sqrt[n]{x^2}\right)^{n/2}\right]^2$
	\begin{enumerate}[label={\Alph*.}]
	\item \(\cfrac{1}{x^2}\)
	\item \(x\)
	\item \(x^2\)
	\item \(x^{\frac{n}{2}}\)
	\end{enumerate}
\item Solve for $x$ if $3^x - 3^{x-1} = 486$
	\begin{enumerate}[label={\Alph*.}]
	\item \(5\)
	\item \(6\)
	\item \(7\)
	\item \(9\)
	\end{enumerate}
\item If $5\sqrt{5} \times 5^3 \div 5^{-\frac{3}{2}} = 5^{a+2}$, then the value of $a$ is 
	\begin{enumerate}[label={\Alph*.}]
	\item \(4\)
	\item \(5\)
	\item \(6\)
	\item \(8\)
	\end{enumerate}
\item If $\left(\sqrt{3}\right)^5 \times 9^2 = 3^n \times 3\sqrt{3}$, then find $n$
	\begin{enumerate}[label={\Alph*.}]
	\item \(2\)
	\item \(3\)
	\item \(4\)
	\item \(5\)
	\end{enumerate}
\item The value of \, $\cfrac{243^{\frac{n}{5}} \times 3^{2n + 1}}{9^n \times 3^{n-1}}$
	\begin{enumerate}[label={\Alph*.}]
	\item \(3\)
	\item \(6\)
	\item \(9\)
	\item \(12\)
	\end{enumerate}
\item If $k^ak^bk^c = 1$, then the value of $a^3 + b^3 + c^3$ is:
	\begin{enumerate}[label={\Alph*.}]
	\item \(9\)
	\item \(a + b + c\)
	\item \(abc\)
	\item \(3abc\)
	\end{enumerate}
\item The value of $\cfrac{81^{3.6} \times 9^{2.7}}{81^{4.2} \times 3}$ is
	\begin{enumerate}[label={\Alph*.}]
	\item \(3\)
	\item \(6\)
	\item \(9\)
	\item \(8.2\)
	\end{enumerate}
\item Simplify $\cfrac{6^{2n +1} \times 9^n \times 4^{2n}}{18^n \times 2^n \times 12^{2n}}$
	\begin{enumerate}[label={\Alph*.}]
	\item \(3^{2n}\)
	\item \(3 \times 2^{n+1}\)
	\item \(2n\)
	\item \(6\)
	\item \(1\)
	\end{enumerate}
\item Solve the systems of equations: $2^{x+y} = 32$  and $3^{3y -x} = 27$, find $(x,y)$ respectively
	\begin{enumerate}[label={\Alph*.}]
	\item \((-3,2)\)
	\item \((-3,-2)\)
	\item \((3,2)\)
	\item \((2,2)\)
	\item \((3,-2)\)
	\end{enumerate}
\item
	\begin{enumerate}[label={\Alph*.}]
	\item \(\)
	\item \(\)
	\item \(\)
	\item \(\)
	\end{enumerate}
\item
	\begin{enumerate}[label={\Alph*.}]
	\item \(\)
	\item \(\)
	\item \(\)
	\item \(\)
	\end{enumerate}
\item
	\begin{enumerate}[label={\Alph*.}]
	\item \(\)
	\item \(\)
	\item \(\)
	\item \(\)
	\end{enumerate}
\item
	\begin{enumerate}[label={\Alph*.}]
	\item \(\)
	\item \(\)
	\item \(\)
	\item \(\)
	\end{enumerate}
\item
	\begin{enumerate}[label={\Alph*.}]
	\item \(\)
	\item \(\)
	\item \(\)
	\item \(\)
	\end{enumerate}
\item
	\begin{enumerate}[label={\Alph*.}]
	\item \(\)
	\item \(\)
	\item \(\)
	\item \(\)
	\end{enumerate}
\item
	\begin{enumerate}[label={\Alph*.}]
	\item \(\)
	\item \(\)
	\item \(\)
	\item \(\)
	\end{enumerate}
\item
	\begin{enumerate}[label={\Alph*.}]
	\item \(\)
	\item \(\)
	\item \(\)
	\item \(\)
	\end{enumerate}
\item
	\begin{enumerate}[label={\Alph*.}]
	\item \(\)
	\item \(\)
	\item \(\)
	\item \(\)
	\end{enumerate}
\item
	\begin{enumerate}[label={\Alph*.}]
	\item \(\)
	\item \(\)
	\item \(\)
	\item \(\)
	\end{enumerate}
\item
	\begin{enumerate}[label={\Alph*.}]
	\item \(\)
	\item \(\)
	\item \(\)
	\item \(\)
	\end{enumerate}
\item
	\begin{enumerate}[label={\Alph*.}]
	\item \(\)
	\item \(\)
	\item \(\)
	\item \(\)
	\end{enumerate}
\item
	\begin{enumerate}[label={\Alph*.}]
	\item \(\)
	\item \(\)
	\item \(\)
	\item \(\)
	\end{enumerate}
\item
	\begin{enumerate}[label={\Alph*.}]
	\item \(\)
	\item \(\)
	\item \(\)
	\item \(\)
	\end{enumerate}
\item
	\begin{enumerate}[label={\Alph*.}]
	\item \(\)
	\item \(\)
	\item \(\)
	\item \(\)
	\end{enumerate}
\item
	\begin{enumerate}[label={\Alph*.}]
	\item \(\)
	\item \(\)
	\item \(\)
	\item \(\)
	\end{enumerate}
\item
	\begin{enumerate}[label={\Alph*.}]
	\item \(\)
	\item \(\)
	\item \(\)
	\item \(\)
	\end{enumerate}
\item
	\begin{enumerate}[label={\Alph*.}]
	\item \(\)
	\item \(\)
	\item \(\)
	\item \(\)
	\end{enumerate}
\item
	\begin{enumerate}[label={\Alph*.}]
	\item \(\)
	\item \(\)
	\item \(\)
	\item \(\)
	\end{enumerate}
\item
	\begin{enumerate}[label={\Alph*.}]
	\item \(\)
	\item \(\)
	\item \(\)
	\item \(\)
	\end{enumerate}
\item
	\begin{enumerate}[label={\Alph*.}]
	\item \(\)
	\item \(\)
	\item \(\)
	\item \(\)
	\end{enumerate}
\item
	\begin{enumerate}[label={\Alph*.}]
	\item \(\)
	\item \(\)
	\item \(\)
	\item \(\)
	\end{enumerate}
\item
	\begin{enumerate}[label={\Alph*.}]
	\item \(\)
	\item \(\)
	\item \(\)
	\item \(\)
	\end{enumerate}
\item
	\begin{enumerate}[label={\Alph*.}]
	\item \(\)
	\item \(\)
	\item \(\)
	\item \(\)
	\end{enumerate}
\item
	\begin{enumerate}[label={\Alph*.}]
	\item \(\)
	\item \(\)
	\item \(\)
	\item \(\)
	\end{enumerate}
\item
	\begin{enumerate}[label={\Alph*.}]
	\item \(\)
	\item \(\)
	\item \(\)
	\item \(\)
	\end{enumerate}
\item
	\begin{enumerate}[label={\Alph*.}]
	\item \(\)
	\item \(\)
	\item \(\)
	\item \(\)
	\end{enumerate}
\item
	\begin{enumerate}[label={\Alph*.}]
	\item \(\)
	\item \(\)
	\item \(\)
	\item \(\)
	\end{enumerate}
\item
	\begin{enumerate}[label={\Alph*.}]
	\item \(\)
	\item \(\)
	\item \(\)
	\item \(\)
	\end{enumerate}
\item
	\begin{enumerate}[label={\Alph*.}]
	\item \(\)
	\item \(\)
	\item \(\)
	\item \(\)
	\end{enumerate}
\item
	\begin{enumerate}[label={\Alph*.}]
	\item \(\)
	\item \(\)
	\item \(\)
	\item \(\)
	\end{enumerate}
\item
	\begin{enumerate}[label={\Alph*.}]
	\item \(\)
	\item \(\)
	\item \(\)
	\item \(\)
	\end{enumerate}
\item
	\begin{enumerate}[label={\Alph*.}]
	\item \(\)
	\item \(\)
	\item \(\)
	\item \(\)
	\end{enumerate}
\item
	\begin{enumerate}[label={\Alph*.}]
	\item \(\)
	\item \(\)
	\item \(\)
	\item \(\)
	\end{enumerate}
\item
	\begin{enumerate}[label={\Alph*.}]
	\item \(\)
	\item \(\)
	\item \(\)
	\item \(\)
	\end{enumerate}
\item
	\begin{enumerate}[label={\Alph*.}]
	\item \(\)
	\item \(\)
	\item \(\)
	\item \(\)
	\end{enumerate}
\item
	\begin{enumerate}[label={\Alph*.}]
	\item \(\)
	\item \(\)
	\item \(\)
	\item \(\)
	\end{enumerate}
\item
	\begin{enumerate}[label={\Alph*.}]
	\item \(\)
	\item \(\)
	\item \(\)
	\item \(\)
	\end{enumerate}


\item
	\begin{enumerate}[label={\Alph*.}]
	\item \(\)
	\item \(\)
	\item \(\)
	\item \(\)
	\end{enumerate}
\item
	\begin{enumerate}[label={\Alph*.}]
	\item \(\)
	\item \(\)
	\item \(\)
	\item \(\)
	\end{enumerate}
\item
	\begin{enumerate}[label={\Alph*.}]
	\item \(\)
	\item \(\)
	\item \(\)
	\item \(\)
	\end{enumerate}
\item
	\begin{enumerate}[label={\Alph*.}]
	\item \(\)
	\item \(\)
	\item \(\)
	\item \(\)
	\end{enumerate}
\item
	\begin{enumerate}[label={\Alph*.}]
	\item \(\)
	\item \(\)
	\item \(\)
	\item \(\)
	\end{enumerate}
\item
	\begin{enumerate}[label={\Alph*.}]
	\item \(\)
	\item \(\)
	\item \(\)
	\item \(\)
	\end{enumerate}
\item
	\begin{enumerate}[label={\Alph*.}]
	\item \(\)
	\item \(\)
	\item \(\)
	\item \(\)
	\end{enumerate}
\item
	\begin{enumerate}[label={\Alph*.}]
	\item \(\)
	\item \(\)
	\item \(\)
	\item \(\)
	\end{enumerate}
\item
	\begin{enumerate}[label={\Alph*.}]
	\item \(\)
	\item \(\)
	\item \(\)
	\item \(\)
	\end{enumerate}
\item
	\begin{enumerate}[label={\Alph*.}]
	\item \(\)
	\item \(\)
	\item \(\)
	\item \(\)
	\end{enumerate}
\item
	\begin{enumerate}[label={\Alph*.}]
	\item \(\)
	\item \(\)
	\item \(\)
	\item \(\)
	\end{enumerate}
\item
	\begin{enumerate}[label={\Alph*.}]
	\item \(\)
	\item \(\)
	\item \(\)
	\item \(\)
	\end{enumerate}
\item
	\begin{enumerate}[label={\Alph*.}]
	\item \(\)
	\item \(\)
	\item \(\)
	\item \(\)
	\end{enumerate}
\item
	\begin{enumerate}[label={\Alph*.}]
	\item \(\)
	\item \(\)
	\item \(\)
	\item \(\)
	\end{enumerate}
\item
	\begin{enumerate}[label={\Alph*.}]
	\item \(\)
	\item \(\)
	\item \(\)
	\item \(\)
	\end{enumerate}
\item
	\begin{enumerate}[label={\Alph*.}]
	\item \(\)
	\item \(\)
	\item \(\)
	\item \(\)
	\end{enumerate}
\item
	\begin{enumerate}[label={\Alph*.}]
	\item \(\)
	\item \(\)
	\item \(\)
	\item \(\)
	\end{enumerate}
\item
	\begin{enumerate}[label={\Alph*.}]
	\item \(\)
	\item \(\)
	\item \(\)
	\item \(\)
	\end{enumerate}
\item
	\begin{enumerate}[label={\Alph*.}]
	\item \(\)
	\item \(\)
	\item \(\)
	\item \(\)
	\end{enumerate}
\item
	\begin{enumerate}[label={\Alph*.}]
	\item \(\)
	\item \(\)
	\item \(\)
	\item \(\)
	\end{enumerate}
\item
	\begin{enumerate}[label={\Alph*.}]
	\item \(\)
	\item \(\)
	\item \(\)
	\item \(\)
	\end{enumerate}
\item
	\begin{enumerate}[label={\Alph*.}]
	\item \(\)
	\item \(\)
	\item \(\)
	\item \(\)
	\end{enumerate}
\item
	\begin{enumerate}[label={\Alph*.}]
	\item \(\)
	\item \(\)
	\item \(\)
	\item \(\)
	\end{enumerate}
\item
	\begin{enumerate}[label={\Alph*.}]
	\item \(\)
	\item \(\)
	\item \(\)
	\item \(\)
	\end{enumerate}
\item
	\begin{enumerate}[label={\Alph*.}]
	\item \(\)
	\item \(\)
	\item \(\)
	\item \(\)
	\end{enumerate}
\end{enumerate}
\end{multicols}