\section{Integration}
\subsection{Questions}
\begin{multicols}{2}
\begin{enumerate}[label={\arabic*.}]
\item Find the integral of \(y = 3{x}^{2}-2x-1\)
	\begin{enumerate}[label={\Alph*.}]
	\item \({x}^{3} - {x}^{2} - x\)
	\item \({x}^{3} + {x}^{2} - x\)
	\item \({x}^{3} + {x}^{2} + x\)
	\item \({x}^{3} - {x}^{2} + x\)
	\end{enumerate}
\item Integrate the expression \(6{x}^{2} - 2x + 1\)
	\begin{enumerate}[label={\Alph*.}]
	\item \(3{x}^{3} - 2{x}^{2} + x + c\)
	\item \(2{x}^{3} - x^{2} + x + c\)
	\item \(2{x}^{3} - 3{x}^{2} + c\)
	\item \({x}^{3} + {x}^{2} - x + c\)
	\end{enumerate}
\item Integrate \(\dfrac{1}{x} + \cos {x}\) with respect to \(x\)
	\begin{enumerate}[label={\Alph*.}]
	\item \(x - \sin {x} + k\)
	\item \(x + \sin {x} - k\)
	\item \(-{\dfrac{1}{x^2}} + \sin {x} + k\)
	\item \(-{\dfrac{1}{x^2}} - \sin {x} + k\)
	\end{enumerate}
\item If the expression \(a{x}^{2} + bx + c\) equals \(5\) at \(x = 1\). If its derivative is \(2x + 1\), what are the values of \(a\),\(b\), \(c\) respectively?
	\begin{enumerate}[label={\Alph*.}]
	\item \(1, 1, 3\)
	\item \(1, 3, 1\)
	\item \(1, 2, 1\)
	\item \(2, 1, 1\)
	\end{enumerate}
\item Integrate the expression \((2x+1)^{3}\)
	\begin{enumerate}[label={\Alph*.}]
	\item \(\dfrac{(2x+1)^{3}}{8} + k\)
	\item \(\dfrac{(2x+1)^{4}}{8} + k\)
	\item \(\dfrac{(2x+1)^{4}}{6} + k\)
	\item \(\dfrac{(2x+1)^{2}}{8} + k\)
	\end{enumerate}
\item Evaluate \(\displaystyle \int 4x^{-3}-7x^{2}+5x-6\ \mathrm{d}x\)
	\begin{enumerate}[label={\Alph*.}]
	\item \(-2x^{-2}-\dfrac{7}{3}x^{3}+\dfrac{5}{2}x^2-6x\)
	\item \(2x^{2}+\dfrac{7}{3}x^{3}+5x^{2}-6\)
	\item \(12x^{2}+14x-5\)
	\item \(-12x^{-4}-14x+5\)
	\end{enumerate}
\item Evaluate \(\displaystyle \int_{-1}^{2}\left(2x^{2} + x\right)\ \mathrm{d}x\)
	\begin{enumerate}[label={\Alph*.}]
	\item \(4\frac{1}{2}\)
	\item \(3\frac{1}{2}\)
	\item \(7\frac{1}{2}\)
	\item \(5\frac{1}{4}\)
	\end{enumerate}
\item Integrate \(\dfrac{x^{2}-\sqrt{x}}{x}\) with respect to \(x\)
	\begin{enumerate}[label={\Alph*.}]
	\item \(\dfrac{x^{2}}{2} - 2\sqrt{x} + k\)
	\item \(\dfrac{2(x^{2}-x)}{3x} + k\)
	\item \(\dfrac{x^{2}}{2} - \sqrt{x} + k\)
	\item \(\dfrac{x^{2}-x}{3x} + k\)
	\end{enumerate}
\item Evaluate \(\displaystyle \int_{-1}^{1} \left(2x + 1\right)^{2}\ \mathrm{d}x\)
	\begin{enumerate}[label={\Alph*.}]
	\item \(3\frac{2}{3}\)
	\item \(4\)
	\item \(4\frac{1}{3}\)
	\item \(4\frac{2}{3}\)
	\end{enumerate}
\item Evaluate \(\displaystyle \int \left(\cos{4x} + \sin{3x}\right)\ \mathrm{d}x\)
	\begin{enumerate}[label={\Alph*.}]
	\item \(\sin{4x} - \cos{3x} + k\)
	\item \(\sin{4x} + \cos{3x} + k\)
	\item \(\cfrac{1}{4}\sin{4x} - \cfrac{1}{3}\cos{3x} + k\)
	\item \(\cfrac{1}{4}\sin{4x} + \cfrac{1}{3}\cos{3x} + k\)
	\end{enumerate}
\item Evaluate \(\displaystyle \int_{0}^{\cfrac{\pi}{2}} \sin{x}\ \mathrm{d}x\)
	\begin{enumerate}[label={\Alph*.}]
	\item \(-2\)
	\item \(-1\)
	\item \(1\)
	\item \(2\)
	\end{enumerate}
\item Evaluate \(\displaystyle \int_{1}^{2}\frac{5}{x}\ \mathrm{d}x\)
	\begin{enumerate}[label={\Alph*.}]
	\item \(1.47\)
	\item \(2.67\)
	\item \(3.23\)
	\item \(3.47\)
	\end{enumerate}
\item Evaluate the integral \(\displaystyle \int_{\frac{\pi}{12}}^{\frac{\pi}{4}} 2\cos{2x}\ \mathrm{d}x\)
	\begin{enumerate}[label={\Alph*.}]
	\item \(-{\frac{1}{2}}\)
	\item \(-1\)
	\item \(\frac{1}{2}\)
	\item \(1\)
	\end{enumerate}
\item Evaluate \(\displaystyle \int \left(2x+3\right)^{\frac{1}{2}}\ \mathrm{d}x\)
	\begin{enumerate}[label={\Alph*.}]
	\item \(\frac{1}{12}(2x+3)^6 + k\)
	\item \(\frac{1}{3}(2x+3)^{\frac{1}{2}} + k\)
	\item \(\frac{1}{3}(2x+3)^{\frac{3}{2}} + k\)
	\item \(\frac{1}{12}(2x+3)^{\frac{3}{4}} + k\)
	\end{enumerate}
\item \item Evaluate \(\displaystyle \int \left(\sin{x} - 5{x}^{2}\right)\ \mathrm{d}x\)
	\begin{enumerate}[label={\Alph*.}]
	\item \(-\cos{x} - 10x + k\)
	\item \(\cos{x} - \cfrac{5x^3}{3} + k\)
	\item \(-\cos{x} - \cfrac{5x^3}{3} + k\)
	\item \(\cos{x} - 10x + k\)
	\end{enumerate}
\item \item Evaluate \(\displaystyle \int \sin{2x}\ \mathrm{d}x\)
	\begin{enumerate}[label={\Alph*.}]
	\item \(\cos{2x} + k\)
	\item \(\cfrac{1}{2}\cos{2x} + k\)
	\item \(-\cfrac{1}{2}\cos{2x} + k\)
	\item \(-\cos{2x} + k\)
	\end{enumerate}
\item If \(y = x(x^4 + x + 1)\), evaluate \(\displaystyle \int_{0}^{1} y\ \mathrm{d}x\)
	\begin{enumerate}[label={\Alph*.}]
	\item \(\frac{11}{12}\)
	\item \(1\)
	\item \(\frac{5}{6}\)
	\item \(0\)
	\end{enumerate}
\item Evaluate \(\displaystyle \int_{2}^{\pi} \sec^{2}{x} - \tan^{2}{x}\ \mathrm{d}x\)
	\begin{enumerate}[label={\Alph*.}]
	\item \(\frac{\pi}{2}\)
	\item \(\frac{\pi}{3}\)
	\item \(\pi - 2\)
	\item \(\pi + 2\)
	\end{enumerate}
\item
	\begin{enumerate}[label={\Alph*.}]
	\item \(\)
	\item \(\)
	\item \(\)
	\item \(\)
	\end{enumerate}
\item
	\begin{enumerate}[label={\Alph*.}]
	\item \(\)
	\item \(\)
	\item \(\)
	\item \(\)
	\end{enumerate}
\item
	\begin{enumerate}[label={\Alph*.}]
	\item \(\)
	\item \(\)
	\item \(\)
	\item \(\)
	\end{enumerate}
\item
	\begin{enumerate}[label={\Alph*.}]
	\item \(\)
	\item \(\)
	\item \(\)
	\item \(\)
	\end{enumerate}
\item
	\begin{enumerate}[label={\Alph*.}]
	\item \(\)
	\item \(\)
	\item \(\)
	\item \(\)
	\end{enumerate}
\item
	\begin{enumerate}[label={\Alph*.}]
	\item \(\)
	\item \(\)
	\item \(\)
	\item \(\)
	\end{enumerate}
\item
	\begin{enumerate}[label={\Alph*.}]
	\item \(\)
	\item \(\)
	\item \(\)
	\item \(\)
	\end{enumerate}
\item
	\begin{enumerate}[label={\Alph*.}]
	\item \(\)
	\item \(\)
	\item \(\)
	\item \(\)
	\end{enumerate}
\item
	\begin{enumerate}[label={\Alph*.}]
	\item \(\)
	\item \(\)
	\item \(\)
	\item \(\)
	\end{enumerate}
\item
	\begin{enumerate}[label={\Alph*.}]
	\item \(\)
	\item \(\)
	\item \(\)
	\item \(\)
	\end{enumerate}
\item
	\begin{enumerate}[label={\Alph*.}]
	\item \(\)
	\item \(\)
	\item \(\)
	\item \(\)
	\end{enumerate}
\item
	\begin{enumerate}[label={\Alph*.}]
	\item \(\)
	\item \(\)
	\item \(\)
	\item \(\)
	\end{enumerate}
\item
	\begin{enumerate}[label={\Alph*.}]
	\item \(\)
	\item \(\)
	\item \(\)
	\item \(\)
	\end{enumerate}
\item
	\begin{enumerate}[label={\Alph*.}]
	\item \(\)
	\item \(\)
	\item \(\)
	\item \(\)
	\end{enumerate}
\item
	\begin{enumerate}[label={\Alph*.}]
	\item \(\)
	\item \(\)
	\item \(\)
	\item \(\)
	\end{enumerate}
\item
	\begin{enumerate}[label={\Alph*.}]
	\item \(\)
	\item \(\)
	\item \(\)
	\item \(\)
	\end{enumerate}
\item
	\begin{enumerate}[label={\Alph*.}]
	\item \(\)
	\item \(\)
	\item \(\)
	\item \(\)
	\end{enumerate}
\item
	\begin{enumerate}[label={\Alph*.}]
	\item \(\)
	\item \(\)
	\item \(\)
	\item \(\)
	\end{enumerate}
\item
	\begin{enumerate}[label={\Alph*.}]
	\item \(\)
	\item \(\)
	\item \(\)
	\item \(\)
	\end{enumerate}
\item
	\begin{enumerate}[label={\Alph*.}]
	\item \(\)
	\item \(\)
	\item \(\)
	\item \(\)
	\end{enumerate}
\item
	\begin{enumerate}[label={\Alph*.}]
	\item \(\)
	\item \(\)
	\item \(\)
	\item \(\)
	\end{enumerate}
\item
	\begin{enumerate}[label={\Alph*.}]
	\item \(\)
	\item \(\)
	\item \(\)
	\item \(\)
	\end{enumerate}
\item
	\begin{enumerate}[label={\Alph*.}]
	\item \(\)
	\item \(\)
	\item \(\)
	\item \(\)
	\end{enumerate}
\item
	\begin{enumerate}[label={\Alph*.}]
	\item \(\)
	\item \(\)
	\item \(\)
	\item \(\)
	\end{enumerate}
\item
	\begin{enumerate}[label={\Alph*.}]
	\item \(\)
	\item \(\)
	\item \(\)
	\item \(\)
	\end{enumerate}
\item
	\begin{enumerate}[label={\Alph*.}]
	\item \(\)
	\item \(\)
	\item \(\)
	\item \(\)
	\end{enumerate}
\item
	\begin{enumerate}[label={\Alph*.}]
	\item \(\)
	\item \(\)
	\item \(\)
	\item \(\)
	\end{enumerate}
\item
	\begin{enumerate}[label={\Alph*.}]
	\item \(\)
	\item \(\)
	\item \(\)
	\item \(\)
	\end{enumerate}
\item
	\begin{enumerate}[label={\Alph*.}]
	\item \(\)
	\item \(\)
	\item \(\)
	\item \(\)
	\end{enumerate}
\item
	\begin{enumerate}[label={\Alph*.}]
	\item \(\)
	\item \(\)
	\item \(\)
	\item \(\)
	\end{enumerate}
\item
	\begin{enumerate}[label={\Alph*.}]
	\item \(\)
	\item \(\)
	\item \(\)
	\item \(\)
	\end{enumerate}
\item
	\begin{enumerate}[label={\Alph*.}]
	\item \(\)
	\item \(\)
	\item \(\)
	\item \(\)
	\end{enumerate}
\item
	\begin{enumerate}[label={\Alph*.}]
	\item \(\)
	\item \(\)
	\item \(\)
	\item \(\)
	\end{enumerate}
\item
	\begin{enumerate}[label={\Alph*.}]
	\item \(\)
	\item \(\)
	\item \(\)
	\item \(\)
	\end{enumerate}
\item
	\begin{enumerate}[label={\Alph*.}]
	\item \(\)
	\item \(\)
	\item \(\)
	\item \(\)
	\end{enumerate}
\item
	\begin{enumerate}[label={\Alph*.}]
	\item \(\)
	\item \(\)
	\item \(\)
	\item \(\)
	\end{enumerate}
\item
	\begin{enumerate}[label={\Alph*.}]
	\item \(\)
	\item \(\)
	\item \(\)
	\item \(\)
	\end{enumerate}
\item
	\begin{enumerate}[label={\Alph*.}]
	\item \(\)
	\item \(\)
	\item \(\)
	\item \(\)
	\end{enumerate}
\item
	\begin{enumerate}[label={\Alph*.}]
	\item \(\)
	\item \(\)
	\item \(\)
	\item \(\)
	\end{enumerate}
\item
	\begin{enumerate}[label={\Alph*.}]
	\item \(\)
	\item \(\)
	\item \(\)
	\item \(\)
	\end{enumerate}
\item
	\begin{enumerate}[label={\Alph*.}]
	\item \(\)
	\item \(\)
	\item \(\)
	\item \(\)
	\end{enumerate}
\item
	\begin{enumerate}[label={\Alph*.}]
	\item \(\)
	\item \(\)
	\item \(\)
	\item \(\)
	\end{enumerate}
\item
	\begin{enumerate}[label={\Alph*.}]
	\item \(\)
	\item \(\)
	\item \(\)
	\item \(\)
	\end{enumerate}
\item
	\begin{enumerate}[label={\Alph*.}]
	\item \(\)
	\item \(\)
	\item \(\)
	\item \(\)
	\end{enumerate}
\item
	\begin{enumerate}[label={\Alph*.}]
	\item \(\)
	\item \(\)
	\item \(\)
	\item \(\)
	\end{enumerate}
\item
	\begin{enumerate}[label={\Alph*.}]
	\item \(\)
	\item \(\)
	\item \(\)
	\item \(\)
	\end{enumerate}
\item
	\begin{enumerate}[label={\Alph*.}]
	\item \(\)
	\item \(\)
	\item \(\)
	\item \(\)
	\end{enumerate}
\item
	\begin{enumerate}[label={\Alph*.}]
	\item \(\)
	\item \(\)
	\item \(\)
	\item \(\)
	\end{enumerate}
\item
	\begin{enumerate}[label={\Alph*.}]
	\item \(\)
	\item \(\)
	\item \(\)
	\item \(\)
	\end{enumerate}
\item
	\begin{enumerate}[label={\Alph*.}]
	\item \(\)
	\item \(\)
	\item \(\)
	\item \(\)
	\end{enumerate}
\item
	\begin{enumerate}[label={\Alph*.}]
	\item \(\)
	\item \(\)
	\item \(\)
	\item \(\)
	\end{enumerate}
\item
	\begin{enumerate}[label={\Alph*.}]
	\item \(\)
	\item \(\)
	\item \(\)
	\item \(\)
	\end{enumerate}
\item
	\begin{enumerate}[label={\Alph*.}]
	\item \(\)
	\item \(\)
	\item \(\)
	\item \(\)
	\end{enumerate}
\item
	\begin{enumerate}[label={\Alph*.}]
	\item \(\)
	\item \(\)
	\item \(\)
	\item \(\)
	\end{enumerate}
\item
	\begin{enumerate}[label={\Alph*.}]
	\item \(\)
	\item \(\)
	\item \(\)
	\item \(\)
	\end{enumerate}
\item
	\begin{enumerate}[label={\Alph*.}]
	\item \(\)
	\item \(\)
	\item \(\)
	\item \(\)
	\end{enumerate}
\item
	\begin{enumerate}[label={\Alph*.}]
	\item \(\)
	\item \(\)
	\item \(\)
	\item \(\)
	\end{enumerate}


\item
	\begin{enumerate}[label={\Alph*.}]
	\item \(\)
	\item \(\)
	\item \(\)
	\item \(\)
	\end{enumerate}
\item
	\begin{enumerate}[label={\Alph*.}]
	\item \(\)
	\item \(\)
	\item \(\)
	\item \(\)
	\end{enumerate}
\item
	\begin{enumerate}[label={\Alph*.}]
	\item \(\)
	\item \(\)
	\item \(\)
	\item \(\)
	\end{enumerate}
\item
	\begin{enumerate}[label={\Alph*.}]
	\item \(\)
	\item \(\)
	\item \(\)
	\item \(\)
	\end{enumerate}
\item
	\begin{enumerate}[label={\Alph*.}]
	\item \(\)
	\item \(\)
	\item \(\)
	\item \(\)
	\end{enumerate}
\item
	\begin{enumerate}[label={\Alph*.}]
	\item \(\)
	\item \(\)
	\item \(\)
	\item \(\)
	\end{enumerate}
\item
	\begin{enumerate}[label={\Alph*.}]
	\item \(\)
	\item \(\)
	\item \(\)
	\item \(\)
	\end{enumerate}
\item
	\begin{enumerate}[label={\Alph*.}]
	\item \(\)
	\item \(\)
	\item \(\)
	\item \(\)
	\end{enumerate}
\item
	\begin{enumerate}[label={\Alph*.}]
	\item \(\)
	\item \(\)
	\item \(\)
	\item \(\)
	\end{enumerate}
\item
	\begin{enumerate}[label={\Alph*.}]
	\item \(\)
	\item \(\)
	\item \(\)
	\item \(\)
	\end{enumerate}
\item
	\begin{enumerate}[label={\Alph*.}]
	\item \(\)
	\item \(\)
	\item \(\)
	\item \(\)
	\end{enumerate}
\item
	\begin{enumerate}[label={\Alph*.}]
	\item \(\)
	\item \(\)
	\item \(\)
	\item \(\)
	\end{enumerate}
\item
	\begin{enumerate}[label={\Alph*.}]
	\item \(\)
	\item \(\)
	\item \(\)
	\item \(\)
	\end{enumerate}
\item
	\begin{enumerate}[label={\Alph*.}]
	\item \(\)
	\item \(\)
	\item \(\)
	\item \(\)
	\end{enumerate}
\item
	\begin{enumerate}[label={\Alph*.}]
	\item \(\)
	\item \(\)
	\item \(\)
	\item \(\)
	\end{enumerate}
\item
	\begin{enumerate}[label={\Alph*.}]
	\item \(\)
	\item \(\)
	\item \(\)
	\item \(\)
	\end{enumerate}
\item
	\begin{enumerate}[label={\Alph*.}]
	\item \(\)
	\item \(\)
	\item \(\)
	\item \(\)
	\end{enumerate}
\item
	\begin{enumerate}[label={\Alph*.}]
	\item \(\)
	\item \(\)
	\item \(\)
	\item \(\)
	\end{enumerate}
\item
	\begin{enumerate}[label={\Alph*.}]
	\item \(\)
	\item \(\)
	\item \(\)
	\item \(\)
	\end{enumerate}
\item
	\begin{enumerate}[label={\Alph*.}]
	\item \(\)
	\item \(\)
	\item \(\)
	\item \(\)
	\end{enumerate}
\item
	\begin{enumerate}[label={\Alph*.}]
	\item \(\)
	\item \(\)
	\item \(\)
	\item \(\)
	\end{enumerate}
\item
	\begin{enumerate}[label={\Alph*.}]
	\item \(\)
	\item \(\)
	\item \(\)
	\item \(\)
	\end{enumerate}
\item
	\begin{enumerate}[label={\Alph*.}]
	\item \(\)
	\item \(\)
	\item \(\)
	\item \(\)
	\end{enumerate}
\item
	\begin{enumerate}[label={\Alph*.}]
	\item \(\)
	\item \(\)
	\item \(\)
	\item \(\)
	\end{enumerate}
\item
	\begin{enumerate}[label={\Alph*.}]
	\item \(\)
	\item \(\)
	\item \(\)
	\item \(\)
	\end{enumerate}
\end{enumerate}
\end{multicols}