\subsection{Solutions}
\begin{enumerate}[label={\textbf{\arabic*.}}]
  \item \textbf{(A)} \(f(-1) = 2(-3)^2 + 7(-3) - 5 = 18 - 21 - 5 = -8\).
  \item \textbf{(D)} \((a^2 - b^2)(x + y) = (a - b)(a + b)(x + y)\).
  \item \textbf{(A)} \(p + q = -7, p - q = -5 \implies 2p = -12 \implies p = -6, q = -1\).
  \item \textbf{(B)} \(f(x) = \frac{1}{x-1} + \frac{1}{x+1} \implies f(1-x) = -\frac{1}{x} - \frac{1}{x-2}\).
  \item \textbf{(D)} Expansion results in \(2x^3 + 6x^2y + 5xy + 15y^2 + 31y + 10x^2 + 2x + 10\).
  \item \textbf{(D)} \(k + l = -7, 4k + l = 5 \implies 3k = 12 \implies k = 4, l = -11\).
  \item \textbf{(E)} \((x - 1)(x + 3)(3x - 2)\).
  \item \textbf{(C)} \((x^2 + x + 1)(x^2 - x + 1) = x^4 + x^2 + 1\).
  \item \textbf{(D)} Roots are \(1, 3, -2\). Other roots are \(3, -2\).
  \item \textbf{(B)} \(l + 2k = -24, -l + k = -3 \implies 3k = -27 \implies k = -9, l = -6\).
  \item \textbf{(E)} \((3a - 2b)(3a + 2b)(9a^2 + 4b^2)\).
  \item \textbf{(D)} Common factor is \(2a + 3b\).
  \item \textbf{(A)} \(p + q = -3\).
  \item \textbf{(B)} \((x - 4)(1 + x)(x - 2)(x - 1)\).
  \item \textbf{(D)} \(f(1) = 4(3)^2 + 3 + 7 = 46\).
  \item \textbf{(C)} \(g(y + 3) = \frac{y}{11} + \frac{11}{y(y + 6)}\).
  \item \textbf{(D)} \((2a + 5x)(4a^2 - 10ax + 25x^2)\).
  \item \textbf{(B)} \((x + 2)(x + a)\).
  \item \textbf{(D)} \(y = x^2 + 3x + 4\) and \(y = \frac{28}{x}\).
  \item \textbf{(A)} \((7a + 1)(a + 5)\).
  \item \textbf{(D)} Roots are \(-2, -2, 4\). Two equal, one different.
  \item \textbf{(D)} \(c = -20, d = -15\).
  \item \textbf{(B)} Common factor is \(1\).
  \item \textbf{(B)} \((x + 1)^2(x - 2)(x + 2)\).
  \item \textbf{(C)} \(f(x + 1) = 2x^2 + 9x + 10\).
  \item \textbf{(A)} \(x^2 + \frac{1}{2}x + \frac{1}{4}\).
  \item \textbf{(D)} \((x + 5y)(5x + y)\).
  \item \textbf{(C)} \((2a - 3b - c)(2a - 3b + c)\).
  \item \textbf{(B)} \(k = -12, l = 4.5\).
  \item \textbf{(C)} \(f(2) = 6^2 + 2(6) + 3 = 51\).
  \item \textbf{(A)} \(y(1 + x)(y + 2)(y - 2)\).
  \item \textbf{(A)} \(2x + 4 = 2(x + 2)\).
  \item \textbf{(D)} \((m - 1)(m + 1)(m - 2)\).
  \item \textbf{(B)} \(r - p\).
  \item \textbf{(B)} \(k = 6\).
  \item \textbf{(C)} \((3p - q + 3r)(3p + q - 3r)\).
  \item \textbf{(B)} \(f(0) = 8\).
  \item \textbf{(C)} \(f(1) = 8\).
  \item \textbf{(B)} \(2(3x + 2)(x - 3)\).
  \item \textbf{(A)} \((ax - 4)(bx - 2y)\).
  \item \textbf{(B)} \((1 - a + b)(1 + a - b)\).
  \item \textbf{(A)} \(x + 3\).
  \item \textbf{(A)} \(x + 7\).
  \item \textbf{(D)} \(p = 2\).
  \item \textbf{(B)} \(p = 2, q = -1\).
  \item \textbf{(A)} \((r - q)(r - 2p)\).
  \item \textbf{(A)} \(x^2 + 5x + 6\).
  \item \textbf{(A)} \((x + y + 6)(x + y - 3)\).
  \item \textbf{(B)} \(2x^2 + x - 1\).
  \item \textbf{(A)} \(a = -1/2, b = 1, c = 1/2\).
  \item \textbf{(B)} \((2x + 5 - 3y)(2x + 5 + 3y)\).
  \item \textbf{(B)} \(a^x - 2\).
  \item \textbf{(A)} \(2, -1, -3\).
  \item \textbf{(A)} \(15x^2 - 11x - 12\).
  \item \textbf{(D)} \(3x - 2y\).
  \item \textbf{(C)} \(\frac{x(x + 5)}{2(x + 2)}\).
  \item \textbf{(C)} \(-73\).
  \item \textbf{(A)} \((a - 2b)(c + a - 2b)\).
  \item \textbf{(B)} \((2y - 3x)(y - 6x)\).
  \item \textbf{(D)} \(k = 1\).
  \item \textbf{(B)} \(3x + 5\).
  \item \textbf{(C)} \(x^3 - 7x - 6 = (x + 2)(x + 1)(x - 3)\).
  \item \textbf{(C)} \(k = -10\).
  \item \textbf{(D)} \(1, -2, 3\).
  \item \textbf{(A)} \((t + 3)(2t - 5)\).
  \item \textbf{(B)} \(k = 5\).
  \item \textbf{(A)} \(-1, 1, -5\).
  \item \textbf{(A)} \(2x - 1\).
  \item \textbf{(D)} \(-178\).
  \item \textbf{(A)} \(16x^2\).
  \item \textbf{(A)} \(5ab(3a - b)^2\).
  \item \textbf{(B)} \(3(a - b)(b - c)(c - a)\).
  \item \textbf{(D)} \((a + 1/a - 1)^2\).
  \item \textbf{(A)} \((5x + 9y)^2\).
  \item \textbf{(B)} \(4a^2\).
  \item \textbf{(C)} \((9xy - 6z)^2\).
  \item \textbf{(A)} \(a = 3\).
  \item \textbf{(B)} \(a = 11/6\).
  \item \textbf{(B)} \(63\).
  \item \textbf{(B)} \((k - p)^2\).
  \item \textbf{(C)} \(m = 6\).
  \item \textbf{(D)} \(x + 7\).
  \item \textbf{(A)} \(a = -4/3\).
  \item \textbf{(D)} \((4x - 9y)(4x - 9y - 3)\).
  \item \textbf{(C)} \((x - 7y)(7x - y)\).
  \item \textbf{(B)} \((a + 1/2)^2\).
  \item \textbf{(B)} \(4b^2\).
  \item \textbf{(C)} \((a + b - 7c)^2\).
  \item \textbf{(A)} \(-\frac{5}{3}x + 12\).
  \item \textbf{(C)} \(a = 7, b = 6\).
  \item \textbf{(D)} \(p = -2, q = 6\).
  \item \textbf{(C)} \(a = 2, b = 12\).
  \item \textbf{(B)} \(a = 2\).
  \item \textbf{(B)} \(2\).
  \item \textbf{(B)} \(m = 9, n = 3\).
  \item \textbf{(A)} Quotient \(4y^2 - 11y + 24\), Remainder \(-52\).
  \item \textbf{(E)} \(c = 5\).
  \item \textbf{(D)} \((x + 1/x)^3\).
  \item \textbf{(D)} \(x + y\).
  \item \textbf{(A)} \(f(b/a)\).
\end{enumerate}
