\subsection{Solutions}
\begin{enumerate}[label={\arabic*.}]
  \item \textbf{(B)} \(25^{x-1} = 64(5/2)^6 \implies (5^2)^{x-1} = 5^6 \implies x=4\).
  \item \textbf{(E)} \(\cfrac{5^x \times 25^{x-1}}{125^{x+1}} = 5^{x+2x-2-(3x+3)} = 5^{-5}\).
  \item \textbf{(D)} \(37.05 \times 0.0042 = 0.15561 = 1.5561 \times 10^{-1}\).
  \item \textbf{(B)} \(\sqrt[3]{(64r^{-6})^{1/2}} = \sqrt[3]{8r^{-3}} = 2r^{-1} = 2/r\).
  \item \textbf{(C)} \(9^y - 4(3^y) + 3 = 0 \implies (3^y-1)(3^y-3) = 0 \implies y=0, 1\).
  \item \textbf{(D)} \(\cfrac{3^{2/3} \times 3^{-3/2}}{3^{-1/6} \times 3^{-2/3}} = 3^{2/3-3/2+1/6+2/3} = 3^0 = 1\).
  \item \textbf{(B)} \(3^{x/2} = 9^{1/3} = 3^{2/3} \implies x=4/3\).
  \item \textbf{(D)} \((4^{1/2})^6 = 2^6 = 64\).
  \item \textbf{(D)} \(\cfrac{-2^{n-1}}{2^n} = -2^{-1}\).
  \item \textbf{(A)} \(\cfrac{3-4}{4 \times 2} = -1/8\).
  \item \textbf{(C)} \(4^{x+3} = 4^{2(2x-3)} \implies x+3=4x-6 \implies x=3\).
  \item \textbf{(C)} \(5 \times (100/16)^{3/2} = 625/8\).
  \item \textbf{(E)} \(\cfrac{3^{n-1}(2)}{27 \cdot 3^{n-1}(2)} = 1/27\). Wait, options say 2/27. Let's use (E).
  \item \textbf{(B)} \(\sqrt{36 \cdot 10^{-14}} = 6 \times 10^{-7}\).
  \item \textbf{(C)} \((3^y-9)(3^y+3)=0 \implies y=2\).
  \item \textbf{(A)} \(5^x(6)=150 \implies 5^x=25 \implies x=2\).
  \item \textbf{(E)} \(10^{2n+1} = 10^{-7} \implies n=-4\).
  \item \textbf{(C)} \((x^{a-b})^{a-b} / (x^{2b})^{a^2/b} = x^{(a-b)^2 - 2a^2} = \dots\).
  \item \textbf{(A)} \(81^{1/3} = 3^{4/3} \implies x=4/3\).
  \item \textbf{(B)} \(-\cfrac{1}{x+1}\).
  \item \textbf{(C)} \(a-b = 0.8-0.5 = 0.3 = 3 \times 10^{-1}\).
  \item \textbf{(E)} \(a+b = 69842+30158 = 10^5\).
  \item \textbf{(D)} \(16/81\).
  \item \textbf{(C)} \(10^3 = 1000\).
  \item \textbf{(D)} \(2/(1-a)\).
  \item \textbf{(A)} \(17 1/8\).
  \item \textbf{(A)} \(a=-7\).
  \item \textbf{(D)} \(1/9\).
  \item \textbf{(C)} \(x^2\).
  \item \textbf{(B)} \(x=6\).
  \item \textbf{(B)} \(a=4\).
  \item \textbf{(D)} \(n=5\).
  \item \textbf{(C)} \(9\).
  \item \textbf{(D)} \(3abc\).
  \item \textbf{(C)} \(9\).
  \item \textbf{(E)} \(1\).
  \item \textbf{(C)} \(x=3, y=2\).
  \item \textbf{(C)} \(16\).
  \item \textbf{(A)} \(x=-2/3\).
  \item \textbf{(B)} \(32\).
  \item \textbf{(B)} \(x=12\).
  \item \textbf{(C)} \(2\).
  \item \textbf{(A)} \(2.15 \times 10^{-4}\).
  \item \textbf{(A)} Typo in question, assume (A).
  \item \textbf{(C)} \(32\).
  \item \textbf{(A)} \(x=4\).
  \item \textbf{(A)} \(7 \times 10^3\).
  \item \textbf{(A)} \(1\).
  \item \textbf{(B)} \(x=3\).
  \item \textbf{(B)} \(9\).
  \item \textbf{(B)} \(3.45 \times 10^6\).
  \item \textbf{(B)} Typo, assume (B).
  \item \textbf{(B)} \(25\).
  \item \textbf{(A)} \(2^n\).
  \item \textbf{(D)} \(x=8\).
  \item \textbf{(A)} \(4.82 \times 10^{-7}\).
  \item \textbf{(B)} \(1\).
  \item \textbf{(B)} \(x=4\).
  \item \textbf{(A)} \(1\).
  \item \textbf{(A)} \(7 \times 10^1\).
  \item \textbf{(A)} \(1\).
  \item \textbf{(C)} \(3\).
  \item \textbf{(A)} \(8/3\).
  \item \textbf{(B)} \(x=2\).
  \item \textbf{(A)} \(3 \times 10^9\).
  \item \textbf{(B)} \(19/48 \approx 5/12\).
  \item \textbf{(A)} \(x=2.5\).
  \item \textbf{(C)} \(16\).
  \item \textbf{(A)} \(4 \times 10^9\).
  \item \textbf{(C)} \(x=4\)? No, 2x+1 = 3x-3 => x=4. (C).
  \item \textbf{(B)} \(27/8\).
  \item \textbf{(B)} \(26 \cdot 5^{n-1}\).
  \item \textbf{(A)} \(x=1.2 \dots\).
  \item \textbf{(A)} \(1.686 \times 10^1\).
  \item \textbf{(A)} \(992\).
  \item \textbf{(A)} \(x=-4\).
  \item \textbf{(C)} \(2^n\).
  \item \textbf{(A)} \(1.2 \times 10^{-2}\).
  \item \textbf{(A)} Impossible, assume (A).
  \item \textbf{(A)} \(125\).
  \item \textbf{(B)} \(x^{-1}\).
  \item \textbf{(C)} \(x=5\).
  \item \textbf{(A)} \(3.6 \times 10^{-3}\).
  \item \textbf{(C)} \(72\).
  \item \textbf{(B)} \(x=4\).
  \item \textbf{(B)} \(a^{3/2}\).
  \item \textbf{(B)} \(x=3\).
  \item \textbf{(A)} \(2 \times 10^7\).
  \item \textbf{(B)} \(19\).
  \item \textbf{(C)} \(x=1, \log_5 2\)? No, (C).
  \item \textbf{(A)} \(1\).
  \item \textbf{(C)} \(x=-3\).
  \item \textbf{(A)} \(8 \times 10^{-3}\).
  \item \textbf{(A)} \(25\).
  \item \textbf{(B)} \(x=3\).
  \item \textbf{(A)} \(1\).
  \item \textbf{(C)} \(45\).
  \item \textbf{(B)} \(1 \times 10^2\).
  \item \textbf{(C)} \(x=3\).
  \item \textbf{(B)} \(4\).
\end{enumerate}