\subsection{Solutions}
\begin{enumerate}[label={\textbf{\arabic*.}}]
  \item \textbf{(A)} \(\int (3x^2-2x-1) dx = x^3 - x^2 - x + C\).

  \item \textbf{(B)} \(\int (6x^2-2x+1) dx = 2x^3 - x^2 + x + c\).

  \item \textbf{(B)} \(\int (x^{-2} + \cos x) dx = -\frac{1}{x} + \sin x + k\).

  \item \textbf{(A)} \(y' = 2x + 1 \implies y = x^2 + x + c\). At \(x=1, y=5 \implies 1+1+c=5 \implies c=3\). \(a=1, b=1, c=3\).

  \item \textbf{(B)} \(\int (2x+1)^3 dx = \frac{(2x+1)^4}{8} + k\).

  \item \textbf{(A)} \(\int (4x^{-3} - 7x^2 + 5x - 6) dx = -2x^{-2} - \frac{7}{3}x^3 + \frac{5}{2}x^2 - 6x + C\).

  \item \textbf{(C)} \(\int_{-1}^2 (2x^2+x) dx = [\frac{2}{3}x^3 + \frac{1}{2}x^2]_{-1}^2 = 7.5\).

  \item \textbf{(A)} \(\int (x - x^{-1/2}) dx = \frac{x^2}{2} - 2\sqrt{x} + k\).

  \item \textbf{(D)} \(\int_{-1}^1 (2x+1)^2 dx = \frac{14}{3} = 4\frac{2}{3}\).

  \item \textbf{(C)} \(\int (\cos 4x + \sin 3x) dx = \frac{1}{4}\sin 4x - \frac{1}{3}\cos 3x + k\).

  \item \textbf{(C)} \(\int_0^{\pi/2} \sin x dx = 1\).

  \item \textbf{(D)} \(\int_1^2 \frac{5}{x} dx = 5\ln 2 \approx 3.47\).

  \item \textbf{(C)} \(\int_{\pi/12}^{\pi/4} 2\cos 2x dx = 0.5\).

  \item \textbf{(C)} \(\int (2x+3)^{1/2} dx = \frac{1}{3}(2x+3)^{3/2} + k\).

  \item \textbf{(C)} \(\int (\sin x - 5x^2) dx = -\cos x - \frac{5}{3}x^3 + k\).

  \item \textbf{(C)} \(\int \sin 2x dx = -\frac{1}{2}\cos 2x + k\).

  \item \textbf{(B)} \(\int_0^1 (x^5+x^2+x) dx = 1\).

  \item \textbf{(C)} \(\int_2^\pi 1 dx = \pi - 2\).

  \item \textbf{(C)} \(\int_0^{\pi/4} (\sin x - \cos x) dx = 1 - \sqrt{2}\).

  \item \textbf{(C)} \(\int_{-2}^1 (x-1)^2 dx = 9\).

  \item \textbf{(A)} \(f(x) = \frac{3}{2}x^2 + 2x\).

  \item \textbf{(C)} \(\int_2^3 (x^2-2x) dx = 4/3\).

  \item \textbf{(D)} \(\int_{-4}^0 (1-2x) dx = 20\).

  \item \textbf{(A)} \(\int_1^2 (6x^2-2x) dx = 11\).

  \item \textbf{(C)} \(\int_{-\pi/2}^{\pi/2} \cos x dx = 2\).

  \item \textbf{(B)} \(\int_0^2 (x^3+x^2) dx = 6\frac{2}{3}\).

  \item \textbf{(C)} \(\int_1^2 2 dx = 2\).

  \item \textbf{(D)} \(\int_1^2 (x^2-4x) dx = -11/3\).

  \item \textbf{(D)} \(\int (\sin x + 2) dx = -\cos x + 2x + k\).

  \item \textbf{(D)} \(\int \cos 4x dx = \frac{1}{4}\sin 4x + k\).

  \item \textbf{(D)} \(\int (x^{-3} + x^{-2}) dx = -\frac{1}{2x^2} - \frac{1}{x} + k\).

  \item \textbf{(C)} \(\int (x^2+3x-5) dx = \frac{x^3}{3} + \frac{3x^2}{2} - 5x + k\).

  \item \textbf{(B)} \(\int (2x^2+2) dx = \frac{2}{3}x^3 + 2x + k\).

  \item \textbf{(B)} \(\int (5x^3 + 7x^2 - 2x + 5) dx = \frac{5}{4}x^4 + \frac{7}{3}x^3 - {x}^2 + 5x + C\).

  \item \textbf{(B)} \(\int_0^\pi -1 d\theta = -\pi\).

  \item \textbf{(C)} \(V = \pi \int_{-1}^3 (y+1) dy = 8\pi \implies K=8\).

  \item \textbf{(B)} \(\int (2x-5)^4 dx = \frac{(2x-5)^5}{10} + C\).

  \item \textbf{(C)} \(\int e^{3x} dx = \frac{1}{3}e^{3x} + C\).

  \item \textbf{(B)} \(\int_0^1 (x^2-x+1) dx = 5/6\).

  \item \textbf{(B)} \(\int \sec^2(3x) dx = \frac{1}{3}\tan 3x + C\).

  \item \textbf{(B)} \(\int_1^e \frac{1}{x} dx = 1\).

  \item \textbf{(C)} Area = \(\int_0^3 x^2 dx = 9\).

  \item \textbf{(A)} \(\int \frac{2}{x+1} dx = 2\ln|x+1| + C\).

  \item \textbf{(B)} \(y = x^2-3x+4\).

  \item \textbf{(A)} \(\int_0^\pi \cos x dx = 0\).

  \item \textbf{(B)} \(\int (3-4x)^{-2} dx = \frac{(3-4x)^{-1}}{4} + C\).

  \item \textbf{(C)} Area = \(\int_{-2}^2 (4-x^2) dx = 32/3\).

  \item \textbf{(C)} \(\int_0^2 (3x^2+4x-5) dx = 6\).

  \item \textbf{(A)} \(\int (x^2-x-2) dx = \frac{x^3}{3} - \frac{x^2}{2} - 2x + C\).

  \item \textbf{(B)} \(\int_1^4 \sqrt{x} dx = 14/3\).

  \item \textbf{(A)} \(y = 2x^2 + 3x\).

  \item \textbf{(A)} \(\int e^{-x/2} dx = -2e^{-x/2} + C\).

  \item \textbf{(B)} Area = \(\int_1^2 x^3 dx = 15/4\).

  \item \textbf{(A)} \(\int_0^{\pi/6} \sec x \tan x dx = \frac{2\sqrt{3}}{3} - 1\).

  \item \textbf{(B)} \(a^2 + a = 4 \implies a \approx 1.56\). Closest is 3/2.

  \item \textbf{(A)} \(\int (1 + x^{-2}) dx = x - \frac{1}{x} + C\).

  \item \textbf{(B)} \(\int (1-x)^3 dx = -\frac{(1-x)^4}{4} + C\).

  \item \textbf{(C)} \(V = \pi \int_0^2 x^2 dx = \frac{8\pi}{3}\).

  \item \textbf{(C)} \(\int_0^{\pi/3} \sin 3x dx = 2/3\).

  \item \textbf{(A)} \(\int (x^4+2x^2+1) dx = \frac{x^5}{5} + \frac{2}{3}x^3 + x + C\).

  \item \textbf{(B)} \(\int_1^k x^{-2} dx = 1/2 \implies k=2\).

  \item \textbf{(A)} \(\int \sec^2 x e^{\tan x} dx = e^{\tan x} + C\).

  \item \textbf{(C)} \(\int \frac{\ln x}{x} dx = \frac{1}{2}(\ln x)^2 + C\).

  \item \textbf{(B)} \(\int_0^1 e^x dx = e - 1\).

  \item \textbf{(B)} \(\int 2^x dx = \frac{2^x}{\ln 2} + C\).

  \item \textbf{(A)} \(\int_0^1 (e^x + e^{-x}) dx = e - 1/e\).

  \item \textbf{(C)} \(\int \frac{1}{2x+3} dx = \frac{1}{2}\ln|2x+3| + C\).

  \item \textbf{(C)} \(\int_0^\pi \sin x dx = 2\).

  \item \textbf{(C)} \(\int x e^{x^2} dx = \frac{1}{2}e^{x^2} + C\).

  \item \textbf{(B)} \(\int_0^{\pi/4} \tan x \sec^2 x dx = 1/2\).

  \item \textbf{(A)} \(\int \cos^2 x dx = \frac{x}{2} + \frac{\sin 2x}{4} + C\).

  \item \textbf{(B)} \(\int_0^b x dx = 8 \implies b=4\).

  \item \textbf{(A)} \(\int \frac{1}{\sqrt{1-x^2}} dx = \arcsin x + C\).

  \item \textbf{(B)} \(V = \pi \int_0^4 x dx = 8\pi\).

  \item \textbf{(A)} \(\int_{-1}^1 x^3 dx = 0\).

  \item \textbf{(B)} \(\int \frac{e^x}{1+e^x} dx = \ln(1+e^x) + C\).

  \item \textbf{(A)} \(\int_1^2 (x + 1/x)^2 dx = 29/6\).

  \item \textbf{(C)} \(y' = \sin x + x \implies y = -\cos x + x^2/2 + 2\).

  \item \textbf{(B)} \(\int 5 dx = 5x + C\).

  \item \textbf{(C)} \(\int_0^2 |x-1| dx = 1\).

  \item \textbf{(B)} \(\int \frac{1}{x \ln x} dx = \ln|\ln x| + C\).

  \item \textbf{(C)} Area = \(\int_1^3 2x dx = 8\).

  \item \textbf{(A)} \(\int \sin^2 x \cos x dx = \frac{\sin^3 x}{3} + C\).

  \item \textbf{(B)} \(\int_e^{e^2} \frac{1}{x \ln x} dx = \ln 2\).

  \item \textbf{(B)} \(\int (x+1)^5 dx = \frac{(x+1)^6}{6} + C\).

  \item \textbf{(A)} \(\int_0^{\pi/2} \cos^3 x \sin x dx = \frac{1}{4}\).

  \item \textbf{(C)} \(\int_0^1 \frac{1}{1+x^2} dx = \pi/4\).

  \item \textbf{(B)} \(\int \sqrt{ax+b} dx = \frac{2}{3a}(ax+b)^{3/2} + C\).

  \item \textbf{(C)} \(f = x^2/2 + 1/x - 1\).

  \item \textbf{(A)} \(\int_{-2}^2 (x^3 + \sin x) dx = 0\).

  \item \textbf{(B)} \(\int x \sqrt{x^2+1} dx = \frac{1}{3}(x^2+1)^{3/2} + C\).

  \item \textbf{(A)} Property: \(\int_a^c f = \int_a^b f + \int_b^c f\).

  \item \textbf{(A)} \(\int (e^{4x} + 2 + e^{-4x}) dx = \frac{1}{4}e^{4x} + 2x - \frac{1}{4}e^{-4x} + C\).

  \item \textbf{(B)} Area = \(\int_0^1 (x - x^2) dx = 1/6\).

  \item \textbf{(B)} \(\int \tan^2 x dx = \tan x - x + C\).

  \item \textbf{(A)} \(\int_0^{\ln 2} e^x dx = 1\).

  \item \textbf{(B)} \(\int \frac{\cos x}{1+\sin^2 x} dx = \arctan(\sin x) + C\).

  \item \textbf{(B)} \(V = \pi \int_1^2 (1/x)^2 dx = \pi/2\).

  \item \textbf{(B)} \(\int \frac{2x+3}{x^2+3x+5} dx = \ln|x^2+3x+5| + C\).

  \item \textbf{(A)} \(\int_0^1 x(x^2+1)^3 dx = 15/8\).
\end{enumerate}