\subsection{Solutions}
\begin{enumerate}[label={\textbf{\arabic*.}}]
  \item \textbf{(B)} \(\log_2 8 = \log_2 2^3 = 3\log_2 2 = 3(1) = 3\).

  \item \textbf{(B)} \(\log_{10} 20 = \log_{10} (2 \times 10) = \log_{10} 2 + \log_{10} 10 = 0.3010 + 1 = 1.3010\).

  \item \textbf{(B)} \(\log_5 125 = \log_5 5^3 = 3\).

  \item \textbf{(A)} \(\log_x 81 = 4 \implies x^4 = 81 = 3^4 \implies x = 3\).

  \item \textbf{(A)} \(\log_3 1 = 0\) (The log of 1 to any base is 0).

  \item \textbf{(C)} \(\log_7 49 + \log_7 7 = \log_7 7^2 + 1 = 2 + 1 = 3\).

  \item \textbf{(C)} \(\log_{10} 50 = \log_{10} (5 \times 10) = \log_{10} 5 + 1 = 0.6990 + 1 = 1.6990\).

  \item \textbf{(B)} \(\log_4 64 = \log_4 4^3 = 3\).

  \item \textbf{(B)} \(\log_2 32 - \log_2 4 = \log_2 2^5 - \log_2 2^2 = 5 - 2 = 3\).

  \item \textbf{(D)} \(\log_5 x = 3 \implies x = 5^3 = 125\).

  \item \textbf{(C)} \(2\log_3 9 = 2\log_3 3^2 = 2(2) = 4\).

  \item \textbf{(C)} \(\log_6 36 + \log_6 1 = 2 + 0 = 2\).

  \item \textbf{(B)} \(\log_{10} 30 = \log_{10} (3 \times 10) = 0.4771 + 1 = 1.4771\).

  \item \textbf{(B)} \(\log_8 512 = \log_8 8^3 = 3\).

  \item \textbf{(B)} \(\log_5 25 \times \log_5 5 = 2 \times 1 = 2\).

  \item \textbf{(C)} \(\log_2 x = 5 \implies x = 2^5 = 32\).

  \item \textbf{(B)} \(\log_{10} 100 = \log_{10} 10^2 = 2\).

  \item \textbf{(B)} \(\log_3 81 - \log_3 9 = 4 - 2 = 2\).

  \item \textbf{(B)} \(\log_{10} 8 = \log_{10} 2^3 = 3\log_{10} 2 = 3(0.3010) = 0.9030\).

  \item \textbf{(B)} \(\log_9 729 = \log_9 9^3 = 3\).

  \item \textbf{(C)} \(3\log_2 4 = 3\log_2 2^2 = 3(2) = 6\).

  \item \textbf{(B)} \(\log_x 16 = 2 \implies x^2 = 16 \implies x = 4\).

  \item \textbf{(A)} \(\log_5 1 = 0\).

  \item \textbf{(B)} \(\log_4 16 + \log_4 4 = 2 + 1 = 3\).

  \item \textbf{(B)} \(\log_{10} 70 = \log_{10} (7 \times 10) = 0.8451 + 1 = 1.8451\).

  \item \textbf{(B)} \(\log_6 216 = \log_6 6^3 = 3\).

  \item \textbf{(B)} \(\log_7 343 - \log_7 49 = 3 - 2 = 1\).

  \item \textbf{(D)} \(\log_3 x = 4 \implies x = 3^4 = 81\).

  \item \textbf{(B)} \(\log_{10} 1000 = 3\).

  \item \textbf{(C)} \(2\log_5 5 + \log_5 25 = 2(1) + 2 = 4\).

  \item \textbf{(A)} \(\log_x 27 = 3 \implies x^3 = 27 = 3^3 \implies x = 3\).

  \item \textbf{(A)} \(\log_2 (1/8) = \log_2 2^{-3} = -3\).

  \item \textbf{(C)} \(\log_3 27 + \log_3 3 = 3 + 1 = 4\).

  \item \textbf{(C)} \(\log_{10} 400 = \log_{10} (4 \times 100) = 0.6021 + 2 = 2.6021\).

  \item \textbf{(A)} \(\log_5 (1/25) = \log_2 5^{-2} = -2\).

  \item \textbf{(B)} \(\log_8 64 - \log_8 8 = 2 - 1 = 1\).

  \item \textbf{(C)} \(\log_4 x = 3 \implies x = 4^3 = 64\).

  \item \textbf{(B)} \(3\log_3 3 = 3(1) = 3\).

  \item \textbf{(C)} \(\log_2 16 + \log_2 2 = 4 + 1 = 5\).

  \item \textbf{(B)} \(\log_{10} 60 = 0.7782 + 1 = 1.7782\).

  \item \textbf{(A)} \(\log_{10} (1/100) = -2\).

  \item \textbf{(B)} \(\log_9 81 + \log_9 9 = 2 + 1 = 3\).

  \item \textbf{(B)} \(\log_7 x = 2 \implies x = 49\).

  \item \textbf{(A)} \(\log_3 (1/27) = -3\).

  \item \textbf{(C)} \(2\log_4 4 + \log_4 16 = 2(1) + 2 = 4\).

  \item \textbf{(B)} \(\log_{10} 800 = 0.9031 + 2 = 2.9031\).

  \item \textbf{(A)} \(\log_6 (1/36) = -2\).

  \item \textbf{(B)} \(\log_{10} 1000 - \log_{10} 10 = 3 - 1 = 2\).

  \item \textbf{(D)} \(\log_2 x = 6 \implies x = 64\).

  \item \textbf{(B)} \(4\log_2 2 = 4(1) = 4\).

  \item \textbf{(C)} \(\log_5 125 + \log_5 5 = 3 + 1 = 4\).

  \item \textbf{(A)} \(\log_x 125 = 3 \implies x = 5\).

  \item \textbf{(A)} \(\log_4 (1/16) = -2\).

  \item \textbf{(B)} \(\log_7 49 + \log_7 7 = 3\).

  \item \textbf{(B)} \(\log_{10} 900 = 0.9542 + 2 = 2.9542\).

  \item \textbf{(A)} \(\log_8 (1/64) = -2\).

  \item \textbf{(B)} \(\log_3 243 - \log_3 27 = 5 - 3 = 2\).

  \item \textbf{(C)} \(\log_6 x = 3 \implies x = 216\).

  \item \textbf{(A)} \(\log_{10} (1/1000) = -3\).

  \item \textbf{(C)} \(3\log_5 5 + \log_5 1 = 3(1) + 0 = 3\).

  \item \textbf{(B)} \(\log_x 64 = 3 \implies x^3 = 64 \implies x = 4\).

  \item \textbf{(A)} \(\log_9 (1/81) = -2\).

  \item \textbf{(B)} \(\log_2 64 + \log_2 4 = 6 + 2 = 8\).

  \item \textbf{(B)} \(\log_8 x = 2 \implies x = 64\).

  \item \textbf{(B)} \(5\log_3 3 = 5\).

  \item \textbf{(B)} \(\log_6 216 - \log_6 36 = 3 - 2 = 1\).

  \item \textbf{(D)} \(\log_{10} x = 2 \implies x = 100\).

  \item \textbf{(A)} \(\log_7 (1/343) = -3\).

  \item \textbf{(C)} \(2\log_6 6 + \log_6 36 = 2 + 2 = 4\).

  \item \textbf{(C)} \(\log_5 x = 4 \implies x = 625\).

  \item \textbf{(A)} \(\log_{10} \sqrt{10} = \frac{1}{2}\).

  \item \textbf{(B)} \(\log_4 256 - \log_4 16 = 4 - 2 = 2\).

  \item \textbf{(A)} \(\log_x 32 = 5 \implies x = 2\).

  \item \textbf{(A)} \(\log_5 (1/125) = -3\).

  \item \textbf{(B)} \(\log_8 512 + \log_8 8 = 3 + 1 = 4\).

  \item \textbf{(B)} \(\log_9 x = 2 \implies x = 81\).

  \item \textbf{(A)} \(\log_{10} \sqrt[3]{10} = \frac{1}{3}\).

  \item \textbf{(C)} \(3\log_2 2 + 2\log_2 4 = 3(1) + 2(2) = 7\).

  \item \textbf{(C)} \(\log_3 x = 5 \implies x = 243\).

  \item \textbf{(A)} \(\log_{10} 0.01 = -2\).

  \item \textbf{(B)} \(\log_5 625 - \log_5 25 = 4 - 2 = 2\).

  \item \textbf{(A)} \(\log_x 1000 = 3 \implies x = 10\).

  \item \textbf{(A)} \(\log_{10} \sqrt[4]{10} = \frac{1}{4}\).

  \item \textbf{(B)} \(\log_7 2401 - \log_7 343 = 4 - 3 = 1\).

  \item \textbf{(D)} \(\log_4 x = 4 \implies x = 256\).

  \item \textbf{(A)} \(\log_{10} 0.001 = -3\).

  \item \textbf{(C)} \(2\log_3 9 + \log_3 3 = 2(2) + 1 = 5\).

  \item \textbf{(B)} \(\log_{10} x = -1 \implies x = 0.1\).

  \item \textbf{(A)} \(\log_2 \sqrt{8} = \log_2 (2^3)^{1/2} = \frac{3}{2}\).

  \item \textbf{(C)} \(\log_9 729 + \log_9 9 = 3 + 1 = 4\).

  \item \textbf{(D)} \(\log_7 x = 3 \implies x = 343\).

  \item \textbf{(A)} \(\log_{10} 0.0001 = -4\).

  \item \textbf{(C)} \(3\log_4 4 + \log_4 64 = 3 + 3 = 6\).

  \item \textbf{(B)} \(\log_{10} x = -2 \implies x = 0.01\).

  \item \textbf{(A)} \(\log_3 \sqrt{27} = \log_3 3^{3/2} = \frac{3}{2}\).

  \item \textbf{(B)} \(\log_{10} 10000 - \log_{10} 100 = 4 - 2 = 2\).

  \item \textbf{(C)} \(\log_2 x = 7 \implies x = 128\).

  \item \textbf{(B)} \(\log_{10} \sqrt{100} = \log_{10} 10 = 1\).

  \item \textbf{(B)} \(\log_6 1296 - \log_6 216 = 4 - 3 = 1\).

  \item \textbf{(A)} \(\log_{10} 18 = \log_{10} (2 \times 3^2) = \log_{10} 2 + 2\log_{10} 3 = 0.3010 + 2(0.4771) = 0.3010 + 0.9542 = 1.2552\).
\end{enumerate}